WIP: more

dataplane/Examples/Label_Propagation_op_Correctness.thy
@@ -1417,6 +1417,49 @@ proof -
     using that[OF cur_t_ts event_le v'_in old_guard updated_guard] .
 qed
 
+lemma label_prop_neighbor_batch_memberD:
+  fixes old_os neighbor_os label_os :: \<open>('d, nat, nat, nat) label_propagation_state\<close>
+  assumes \<open>(x, cap) \<in> set (label_prop_neighbor_batch old_os neighbor_os label_os
+    relevant_times vertex new_label event_time)\<close>
+  obtains cur_t where
+    \<open>cur_t \<in> set relevant_times\<close>
+    \<open>cap = Cap (MyPair cur_t (mysnd event_time)) 1\<close>
+  using assms unfolding label_prop_neighbor_batch_def
+  by (auto simp: Let_def split: if_splits)
+
+lemma label_prop_label_batch_memberD:
+  fixes old_os updated_os :: \<open>('d, nat, nat, nat) label_propagation_state\<close>
+  assumes \<open>(x, cap) \<in> set (label_prop_label_batch old_os updated_os event_t vertex new_label event_time)\<close>
+  obtains cur_t where
+    \<open>cur_t \<in> set (timestamps old_os)\<close>
+    \<open>event_t \<le> cur_t\<close>
+    \<open>cap = Cap (MyPair cur_t (mysnd event_time)) 1\<close>
+proof -
+  obtain cur_t where cur_t_in: \<open>cur_t \<in> set (filter ((\<le>) event_t) (timestamps old_os))\<close>
+    and cap_eq: \<open>cap = Cap (MyPair cur_t (mysnd event_time)) 1\<close>
+    using assms unfolding label_prop_label_batch_def
+    by (elim label_prop_neighbor_batch_memberD)
+  show ?thesis
+    using that cur_t_in cap_eq by auto
+qed
+
+lemma label_prop_input1_step_batch_memberD:
+  fixes os :: \<open>('d, nat, nat, nat) label_propagation_state\<close>
+  assumes \<open>(x, cap) \<in> set (label_prop_input1_step_batch os d t)\<close>
+  obtains cur_t where
+    \<open>cur_t \<in> set (timestamps os)\<close>
+    \<open>myfst t \<le> cur_t\<close>
+    \<open>cap = Cap (MyPair cur_t (mysnd t)) 1\<close>
+proof -
+  obtain cur_t where cur_t_in: \<open>cur_t \<in> set (timestamps os)\<close>
+    and time_le: \<open>myfst t \<le> cur_t\<close>
+    and cap_eq: \<open>cap = Cap (MyPair cur_t (mysnd t)) 1\<close>
+    using assms unfolding label_prop_input1_step_batch_def Let_def
+    by (elim label_prop_label_batch_memberD)
+  show ?thesis
+    using that[OF cur_t_in time_le cap_eq] .
+qed
+
 
 lemma label_prop_input1_step_batch_unfold:
   \<open>label_prop_input1_step_batch os d t =
@@ -1569,6 +1612,38 @@ next
   qed
 qed
 
+
+lemma label_prop_input1_batched_produced_memberD:
+  fixes os :: \<open>('d, nat, nat, nat) label_propagation_state\<close>
+  assumes \<open>(p, pt, n) \<in> set (map (\<lambda>(x, cap). case cap of Cap t p \<Rightarrow> (p, t, 1))
+    (snd (label_prop_input1_batched os msgs)))\<close>
+  obtains
+    \<open>p = 1\<close>
+    \<open>n = 1\<close>
+    \<open>myfst pt \<in> set (timestamps os)\<close>
+    \<open>MyPair (myfst pt) 0 \<le> pt\<close>
+proof -
+  obtain x cap where batch_member: \<open>(x, cap) \<in> set (snd (label_prop_input1_batched os msgs))\<close>
+    and triple_eq: \<open>(p, pt, n) = (case cap of Cap t p \<Rightarrow> (p, t, 1))\<close>
+    using assms by auto
+  obtain pre d t post os_pre where os_pre_eq:
+    \<open>os_pre = fst (label_prop_input1_batched os pre)\<close>
+    and step_member: \<open>(x, cap) \<in> set (label_prop_input1_step_batch os_pre d t)\<close>
+    using batch_member by (elim label_prop_input1_batched_batch_memberD)
+  obtain cur_t where cur_t_pre: \<open>cur_t \<in> set (timestamps os_pre)\<close>
+    and cap_eq: \<open>cap = Cap (MyPair cur_t (mysnd t)) 1\<close>
+    using step_member by (elim label_prop_input1_step_batch_memberD)
+  have cur_t: \<open>cur_t \<in> set (timestamps os)\<close>
+    using cur_t_pre os_pre_eq by simp
+  have fields: \<open>p = 1\<close> \<open>n = 1\<close> \<open>pt = MyPair cur_t (mysnd t)\<close>
+    using triple_eq cap_eq by simp_all
+  have pt_ts: \<open>myfst pt \<in> set (timestamps os)\<close>
+    using fields cur_t by simp
+  have pt_ge: \<open>MyPair (myfst pt) 0 \<le> pt\<close>
+    using fields by simp
+  show ?thesis
+    using that[OF fields(1) fields(2) pt_ts pt_ge] .
+qed
 
 
 lemma outpu_fst_label_prop_input1_batched_nonemptyD:
@@ -2544,16 +2619,16 @@ lemma label_prop_input1_loop_updates_timestmaps:
 
 function loop_updates where
   "loop_updates (cbufs :: 3 \<times> 2 \<Rightarrow> ((nat \<times> nat + nat set set) \<times> (nat, nat) myprod) buf) os_label_prop (os :: 3 \<Rightarrow> (2, nat \<times> nat + nat set set, (nat, nat) myprod) operator_state) = (
-   if \<not> label_prop_upd_inv os_label_prop \<or> \<not> (\<forall> t. labels_inv (all_edges os_label_prop t) (min_label os_label_prop t)) \<or>
-      \<not> (myfst ` snd ` set (input os_label_prop 1 @ outpu os_label_prop 1 @ input (os 2) 1 @ outpu (os 2) 1 @ cbufs (1, 1) @ cbufs (2, 1)) \<subseteq> set (timestamps os_label_prop))
-   then (cbufs((2, 1) := [], (1, 1) := []), os_label_prop, os)
-   else
-   let (cbufs', os_label_prop', os') = label_prop_input1_loop_updates cbufs os_label_prop os in
-   if input os_label_prop' 1 = []
-   then (cbufs', os_label_prop', os')
-   else 
-   loop_updates cbufs' os_label_prop' os'
+   if label_prop_upd_inv os_label_prop \<and> (\<forall> t. labels_inv (all_edges os_label_prop t) (min_label os_label_prop t)) \<and>
+      (myfst ` snd ` set (input os_label_prop 1 @ outpu os_label_prop 1 @ input (os 2) 1 @ outpu (os 2) 1 @ cbufs (1, 1) @ cbufs (2, 1)) \<subseteq> set (timestamps os_label_prop))
+   then
+     let (cbufs', os_label_prop', os') = label_prop_input1_loop_updates cbufs os_label_prop os in
+     if input os_label_prop' 1 = []
+     then (cbufs', os_label_prop', os')
+     else loop_updates cbufs' os_label_prop' os'
+   else (cbufs((2, 1) := [], (1, 1) := []), os_label_prop, os)
    )"
+
   by auto
 termination
   apply (relation "measure (\<lambda>(cbufs, os_label_prop, os). sum_list (map (\<lambda> t. labels_measure (all_edges os_label_prop t) (min_label os_label_prop t)) (timestamps os_label_prop))) ")
@@ -2731,17 +2806,293 @@ proof (induct cbufs os_label_prop os rule: loop_updates.induct)
     by simp
   have ih_applied:
     \<open>input os_label_prop' 1 \<noteq> [] \<Longrightarrow>
-     \<not> (\<not> label_prop_upd_inv os_label_prop \<or>
-        \<not> (\<forall>t. labels_inv (all_edges os_label_prop t) (min_label os_label_prop t)) \<or>
-        \<not> myfst ` snd ` set (input os_label_prop 1 @ outpu os_label_prop 1 @
-              input (os 2) 1 @ outpu (os 2) 1 @ cbufs (1, 1) @ cbufs (2, 1))
-            \<subseteq> set (timestamps os_label_prop)) \<Longrightarrow>
+     label_prop_upd_inv os_label_prop \<and>
+     (\<forall>t. labels_inv (all_edges os_label_prop t) (min_label os_label_prop t)) \<and>
+     myfst ` snd ` set (input os_label_prop 1 @ outpu os_label_prop 1 @
+       input (os 2) 1 @ outpu (os 2) 1 @ cbufs (1, 1) @ cbufs (2, 1))
+       \<subseteq> set (timestamps os_label_prop) \<Longrightarrow>
      fst (loop_updates (cbufs((2, 1) := [], (1, 1) := [])) os_label_prop' os')
        = cbufs((2, 1) := [], (1, 1) := [])\<close>
+
     using 1(1)[OF _ triple[symmetric] refl refl] cbufs'_eq idemp_eq by metis
   show ?case
     by (subst loop_updates.simps) (auto simp: triple cbufs'_eq ih_applied)
 qed
+
+lemma produ_fst_snd_label_prop_input1_loop_updates:
+  fixes os :: \<open>3 \<Rightarrow> (2, 'd, (nat, nat) myprod) operator_state\<close>
+    and os_label_prop :: \<open>('d, nat, nat, nat) label_propagation_state\<close>
+    and os_label_prop_consumed :: \<open>('d, nat, nat, nat) label_propagation_state\<close>
+    and cbufs :: \<open>3 \<times> 2 \<Rightarrow> ('d \<times> (nat, nat) myprod) buf\<close>
+  assumes os_label_prop_consumed_def:
+    \<open>os_label_prop_consumed =
+      CONSUMES 1
+        (cbufs (1, 1) @ outpu (os 2) 1 @
+          map (\<lambda>(d, t). (d, t -+- MyPair 0 (Suc 0)))
+            (input (os 2) 1 @ cbufs (2, 1) @ outpu os_label_prop 1))
+        (os_label_prop\<lparr>outpu := (outpu os_label_prop)(1 := [])\<rparr>)\<close>
+  shows \<open>produ (fst (snd (label_prop_input1_loop_updates cbufs os_label_prop os))) =
+    produ os_label_prop @
+      map (\<lambda>(x, cap). case cap of Cap t p \<Rightarrow> (p, t, 1))
+        (snd (label_prop_input1_batched os_label_prop_consumed (input os_label_prop_consumed 1)))\<close>
+  using os_label_prop_consumed_def
+  unfolding label_prop_input1_loop_updates_def Let_def
+  by (simp add: fold_consumes split_beta split: capability.splits)
+
+
+lemma produ_fst_snd_loop_updates_prefix:
+  fixes os :: \<open>3 \<Rightarrow> (2, nat \<times> nat + nat set set, (nat, nat) myprod) operator_state\<close>
+    and os_label_prop :: \<open>(nat \<times> nat + nat set set, nat, nat, nat) label_propagation_state\<close>
+    and cbufs :: \<open>3 \<times> 2 \<Rightarrow> ((nat \<times> nat + nat set set) \<times> (nat, nat) myprod) buf\<close>
+  obtains produced where
+    \<open>produ (fst (snd (loop_updates cbufs os_label_prop os))) = produ os_label_prop @ produced\<close>
+    \<open>\<forall>p pt n. (p, pt, n) \<in> set produced \<longrightarrow>
+      p = 1 \<and> n = 1 \<and> myfst pt \<in> set (timestamps os_label_prop) \<and> MyPair (myfst pt) 0 \<le> pt\<close>
+proof (induct cbufs os_label_prop os arbitrary: thesis rule: loop_updates.induct)
+  case (1 cbufs os_label_prop os)
+  let ?good = \<open>label_prop_upd_inv os_label_prop \<and>
+    (\<forall>t. labels_inv (all_edges os_label_prop t) (min_label os_label_prop t)) \<and>
+    myfst ` snd ` set (input os_label_prop 1 @ outpu os_label_prop 1 @
+      input (os 2) 1 @ outpu (os 2) 1 @ cbufs (1, 1) @ cbufs (2, 1))
+      \<subseteq> set (timestamps os_label_prop)\<close>
+  show ?case
+  proof (cases ?good)
+    case False
+    have loop_eq: \<open>loop_updates cbufs os_label_prop os =
+      (cbufs((2, 1) := [], (1, 1) := []), os_label_prop, os)\<close>
+      by (subst loop_updates.simps) (use False in auto)
+    show ?thesis
+    proof (rule "1.prems"[of Nil])
+      show \<open>produ (fst (snd (loop_updates cbufs os_label_prop os))) = produ os_label_prop @ []\<close>
+        using loop_eq by simp
+      show \<open>\<forall>p pt n. (p, pt, n) \<in> set [] \<longrightarrow>
+        p = 1 \<and> n = 1 \<and> myfst pt \<in> set (timestamps os_label_prop) \<and> MyPair (myfst pt) 0 \<le> pt\<close>
+        by simp
+    qed
+  next
+    case True
+    obtain cbufs' :: \<open>3 \<times> 2 \<Rightarrow> ((nat \<times> nat + nat set set) \<times> (nat, nat) myprod) buf\<close>
+      and os_label_prop' :: \<open>(nat \<times> nat + nat set set, nat, nat, nat) label_propagation_state\<close>
+      and os' :: \<open>3 \<Rightarrow> (2, nat \<times> nat + nat set set, (nat, nat) myprod) operator_state\<close>
+      where step: \<open>label_prop_input1_loop_updates cbufs os_label_prop os = (cbufs', os_label_prop', os')\<close>
+      by (cases \<open>label_prop_input1_loop_updates cbufs os_label_prop os\<close>) auto
+    let ?msgs = \<open>cbufs (1, 1) @ outpu (os 2) 1 @
+      map (\<lambda>(d, t). (d, t -+- MyPair 0 (Suc 0)))
+        (input (os 2) 1 @ cbufs (2, 1) @ outpu os_label_prop 1)\<close>
+    let ?consumed = \<open>CONSUMES 1 ?msgs (os_label_prop\<lparr>outpu := (outpu os_label_prop)(1 := [])\<rparr>)\<close>
+    let ?produced1 = \<open>map (\<lambda>(x, cap). case cap of Cap t p \<Rightarrow> (p, t, 1))
+      (snd (label_prop_input1_batched ?consumed (input ?consumed 1)))\<close>
+    have consumed_ts: \<open>timestamps ?consumed = timestamps os_label_prop\<close>
+      by simp
+    have produced1_props: \<open>\<forall>p pt n. (p, pt, n) \<in> set ?produced1 \<longrightarrow>
+      p = 1 \<and> n = 1 \<and> myfst pt \<in> set (timestamps os_label_prop) \<and> MyPair (myfst pt) 0 \<le> pt\<close>
+    proof (intro allI impI)
+      fix p pt n
+      assume \<open>(p, pt, n) \<in> set ?produced1\<close>
+      then show \<open>p = 1 \<and> n = 1 \<and> myfst pt \<in> set (timestamps os_label_prop) \<and> MyPair (myfst pt) 0 \<le> pt\<close>
+        by (elim label_prop_input1_batched_produced_memberD) (simp add: consumed_ts)
+    qed
+    have step_prod0:
+      \<open>produ (fst (snd (label_prop_input1_loop_updates cbufs os_label_prop os))) =
+        produ os_label_prop @ ?produced1\<close>
+      unfolding label_prop_input1_loop_updates_def Let_def
+      by (simp add: fold_consumes split_beta split: capability.splits)
+    have step_prod: \<open>produ os_label_prop' = produ os_label_prop @ ?produced1\<close>
+      using step_prod0 step by simp
+    have step_os_label_prop':
+      \<open>os_label_prop' = fst (snd (label_prop_input1_loop_updates cbufs os_label_prop os))\<close>
+      using step by simp
+    have step_ts: \<open>timestamps os_label_prop' = timestamps os_label_prop\<close>
+      using step_os_label_prop'
+      unfolding label_prop_input1_loop_updates_def Let_def
+      by (simp add: fold_consumes split_beta)
+    show ?thesis
+    proof (cases \<open>input os_label_prop' 1 = []\<close>)
+      case True
+      have loop_eq: \<open>loop_updates cbufs os_label_prop os = (cbufs', os_label_prop', os')\<close>
+        by (subst loop_updates.simps) (use \<open>?good\<close> step True in auto)
+      show ?thesis
+      proof (rule "1.prems"[of \<open>?produced1 @ []\<close>])
+        show \<open>produ (fst (snd (loop_updates cbufs os_label_prop os))) =
+          produ os_label_prop @ (?produced1 @ [])\<close>
+          using loop_eq step_prod by simp
+        show \<open>\<forall>p pt n. (p, pt, n) \<in> set (?produced1 @ []) \<longrightarrow>
+          p = 1 \<and> n = 1 \<and> myfst pt \<in> set (timestamps os_label_prop) \<and> MyPair (myfst pt) 0 \<le> pt\<close>
+          using produced1_props by simp
+      qed
+    next
+      case False
+      obtain produced2 where rec_prod:
+        \<open>produ (fst (snd (loop_updates cbufs' os_label_prop' os'))) =
+          produ os_label_prop' @ produced2\<close>
+        and rec_props: \<open>\<forall>p pt n. (p, pt, n) \<in> set produced2 \<longrightarrow>
+          p = 1 \<and> n = 1 \<and> myfst pt \<in> set (timestamps os_label_prop') \<and> MyPair (myfst pt) 0 \<le> pt\<close>
+        using "1.hyps"[OF \<open>?good\<close> step[symmetric] refl refl False]
+        by blast
+      have loop_eq: \<open>loop_updates cbufs os_label_prop os = loop_updates cbufs' os_label_prop' os'\<close>
+        by (subst loop_updates.simps) (use \<open>?good\<close> step False in auto)
+      show ?thesis
+      proof (rule "1.prems"[of \<open>?produced1 @ produced2\<close>])
+        show \<open>produ (fst (snd (loop_updates cbufs os_label_prop os))) =
+          produ os_label_prop @ (?produced1 @ produced2)\<close>
+          using loop_eq rec_prod step_prod by (simp add: append_assoc)
+        show \<open>\<forall>p pt n. (p, pt, n) \<in> set (?produced1 @ produced2) \<longrightarrow>
+          p = 1 \<and> n = 1 \<and> myfst pt \<in> set (timestamps os_label_prop) \<and> MyPair (myfst pt) 0 \<le> pt\<close>
+          using produced1_props rec_props step_ts by auto
+      qed
+    qed
+  qed
+qed
+
+
+lemma produ_fst_snd_loop_updatesE:
+  fixes os :: \<open>3 \<Rightarrow> (2, nat \<times> nat + nat set set, (nat, nat) myprod) operator_state\<close>
+    and os_label_prop :: \<open>(nat \<times> nat + nat set set, nat, nat, nat) label_propagation_state\<close>
+    and os_label_prop_consumed :: \<open>(nat \<times> nat + nat set set, nat, nat, nat) label_propagation_state\<close>
+    and cbufs :: \<open>3 \<times> 2 \<Rightarrow> ((nat \<times> nat + nat set set) \<times> (nat, nat) myprod) buf\<close>
+  assumes INV: \<open>label_prop_upd_inv os_label_prop\<close>
+    and LABELS: \<open>\<forall>t. labels_inv (all_edges os_label_prop t) (min_label os_label_prop t)\<close>
+    and TIMES: \<open>myfst ` snd ` set (input os_label_prop 1 @ outpu os_label_prop 1 @
+        input (os 2) 1 @ outpu (os 2) 1 @ cbufs (1, 1) @ cbufs (2, 1))
+      \<subseteq> set (timestamps os_label_prop)\<close>
+    and os_label_prop_consumed_def:
+    \<open>os_label_prop_consumed =
+      CONSUMES 1
+        (cbufs (1, 1) @ outpu (os 2) 1 @
+          map (\<lambda>(d, t). (d, t -+- MyPair 0 (Suc 0)))
+            (input (os 2) 1 @ cbufs (2, 1) @ outpu os_label_prop 1))
+        (os_label_prop\<lparr>outpu := (outpu os_label_prop)(1 := [])\<rparr>)\<close>
+  obtains produced where
+    \<open>produ (fst (snd (loop_updates cbufs os_label_prop os))) =
+      produ os_label_prop @
+        map (\<lambda>(x, cap). case cap of Cap t p \<Rightarrow> (p, t, 1))
+          (snd (label_prop_input1_batched os_label_prop_consumed (input os_label_prop_consumed 1))) @
+        produced\<close>
+    \<open>\<forall>p pt n. (p, pt, n) \<in> set (
+        map (\<lambda>(x, cap). case cap of Cap t p \<Rightarrow> (p, t, 1))
+          (snd (label_prop_input1_batched os_label_prop_consumed (input os_label_prop_consumed 1))) @ produced) \<longrightarrow>
+      p = 1 \<and> n = 1 \<and> myfst pt \<in> set (timestamps os_label_prop_consumed) \<and> MyPair (myfst pt) 0 \<le> pt\<close>
+proof -
+  let ?good = \<open>label_prop_upd_inv os_label_prop \<and>
+    (\<forall>t. labels_inv (all_edges os_label_prop t) (min_label os_label_prop t)) \<and>
+    myfst ` snd ` set (input os_label_prop 1 @ outpu os_label_prop 1 @
+      input (os 2) 1 @ outpu (os 2) 1 @ cbufs (1, 1) @ cbufs (2, 1))
+      \<subseteq> set (timestamps os_label_prop)\<close>
+  have good: ?good
+    using INV LABELS TIMES by simp
+  obtain cbufs' :: \<open>3 \<times> 2 \<Rightarrow> ((nat \<times> nat + nat set set) \<times> (nat, nat) myprod) buf\<close>
+    and os_label_prop' :: \<open>(nat \<times> nat + nat set set, nat, nat, nat) label_propagation_state\<close>
+    and os' :: \<open>3 \<Rightarrow> (2, nat \<times> nat + nat set set, (nat, nat) myprod) operator_state\<close>
+    where step: \<open>label_prop_input1_loop_updates cbufs os_label_prop os = (cbufs', os_label_prop', os')\<close>
+    by (cases \<open>label_prop_input1_loop_updates cbufs os_label_prop os\<close>) auto
+  let ?produced1 = \<open>map (\<lambda>(x, cap). case cap of Cap t p \<Rightarrow> (p, t, 1))
+    (snd (label_prop_input1_batched os_label_prop_consumed (input os_label_prop_consumed 1)))\<close>
+  have consumed_ts: \<open>timestamps os_label_prop_consumed = timestamps os_label_prop\<close>
+    using os_label_prop_consumed_def by simp
+  have produced1_props: \<open>\<forall>p pt n. (p, pt, n) \<in> set ?produced1 \<longrightarrow>
+    p = 1 \<and> n = 1 \<and> myfst pt \<in> set (timestamps os_label_prop_consumed) \<and> MyPair (myfst pt) 0 \<le> pt\<close>
+  proof (intro allI impI)
+    fix p pt n
+    assume \<open>(p, pt, n) \<in> set ?produced1\<close>
+    then show \<open>p = 1 \<and> n = 1 \<and> myfst pt \<in> set (timestamps os_label_prop_consumed) \<and> MyPair (myfst pt) 0 \<le> pt\<close>
+      by (elim label_prop_input1_batched_produced_memberD) simp
+  qed
+  have step_prod0:
+    \<open>produ (fst (snd (label_prop_input1_loop_updates cbufs os_label_prop os))) =
+      produ os_label_prop @ ?produced1\<close>
+    using os_label_prop_consumed_def
+    unfolding label_prop_input1_loop_updates_def Let_def
+    by (simp add: fold_consumes split_beta split: capability.splits)
+  have step_prod: \<open>produ os_label_prop' = produ os_label_prop @ ?produced1\<close>
+    using step_prod0 step by simp
+  have step_os_label_prop':
+    \<open>os_label_prop' = fst (snd (label_prop_input1_loop_updates cbufs os_label_prop os))\<close>
+    using step by simp
+  have step_ts: \<open>timestamps os_label_prop' = timestamps os_label_prop_consumed\<close>
+    using step_os_label_prop' os_label_prop_consumed_def
+    unfolding label_prop_input1_loop_updates_def Let_def
+    by (simp add: fold_consumes split_beta)
+  show ?thesis
+  proof (cases \<open>input os_label_prop' 1 = []\<close>)
+    case True
+    have \<open>loop_updates cbufs os_label_prop os = (cbufs', os_label_prop', os')\<close>
+      by (subst loop_updates.simps) (use good step True in auto)
+    then have prod_eq: \<open>produ (fst (snd (loop_updates cbufs os_label_prop os))) =
+      produ os_label_prop @ ?produced1 @ []\<close>
+      using step_prod by simp
+    show ?thesis
+      by (rule that[OF prod_eq]) (use produced1_props in simp)
+  next
+    case False
+    obtain produced2 where rec_prod:
+      \<open>produ (fst (snd (loop_updates cbufs' os_label_prop' os'))) =
+        produ os_label_prop' @ produced2\<close>
+      and rec_props: \<open>\<forall>p pt n. (p, pt, n) \<in> set produced2 \<longrightarrow>
+        p = 1 \<and> n = 1 \<and> myfst pt \<in> set (timestamps os_label_prop') \<and> MyPair (myfst pt) 0 \<le> pt\<close>
+      by (elim produ_fst_snd_loop_updates_prefix)
+    have \<open>loop_updates cbufs os_label_prop os = loop_updates cbufs' os_label_prop' os'\<close>
+      by (subst loop_updates.simps) (use good step False in auto)
+    then have prod_eq: \<open>produ (fst (snd (loop_updates cbufs os_label_prop os))) =
+      produ os_label_prop @ ?produced1 @ produced2\<close>
+      using rec_prod step_prod by (simp add: append_assoc)
+    have props: \<open>\<forall>p pt n. (p, pt, n) \<in> set (?produced1 @ produced2) \<longrightarrow>
+      p = 1 \<and> n = 1 \<and> myfst pt \<in> set (timestamps os_label_prop_consumed) \<and> MyPair (myfst pt) 0 \<le> pt\<close>
+      using produced1_props rec_props step_ts by auto
+    show ?thesis
+      by (rule that[OF prod_eq props])
+  qed
+qed
+
+lemma produ_fst_snd_loop_updates:
+  fixes os :: \<open>3 \<Rightarrow> (2, nat \<times> nat + nat set set, (nat, nat) myprod) operator_state\<close>
+    and os_label_prop :: \<open>(nat \<times> nat + nat set set, nat, nat, nat) label_propagation_state\<close>
+    and os_label_prop_consumed :: \<open>(nat \<times> nat + nat set set, nat, nat, nat) label_propagation_state\<close>
+    and cbufs :: \<open>3 \<times> 2 \<Rightarrow> ((nat \<times> nat + nat set set) \<times> (nat, nat) myprod) buf\<close>
+  assumes INV: \<open>label_prop_upd_inv os_label_prop\<close>
+    and LABELS: \<open>\<forall>t. labels_inv (all_edges os_label_prop t) (min_label os_label_prop t)\<close>
+    and TIMES: \<open>myfst ` snd ` set (input os_label_prop 1 @ outpu os_label_prop 1 @
+        input (os 2) 1 @ outpu (os 2) 1 @ cbufs (1, 1) @ cbufs (2, 1))
+      \<subseteq> set (timestamps os_label_prop)\<close>
+    and os_label_prop_consumed_def:
+    \<open>os_label_prop_consumed =
+      CONSUMES 1
+        (cbufs (1, 1) @ outpu (os 2) 1 @
+          map (\<lambda>(d, t). (d, t -+- MyPair 0 (Suc 0)))
+            (input (os 2) 1 @ cbufs (2, 1) @ outpu os_label_prop 1))
+        (os_label_prop\<lparr>outpu := (outpu os_label_prop)(1 := [])\<rparr>)\<close>
+  shows \<open>\<exists>produced.
+    produ (fst (snd (loop_updates cbufs os_label_prop os))) =
+      produ os_label_prop @
+        map (\<lambda>(x, cap). case cap of Cap t p \<Rightarrow> (p, t, 1))
+          (snd (label_prop_input1_batched os_label_prop_consumed (input os_label_prop_consumed 1))) @
+        produced \<and>
+    (\<forall>p pt n. (p, pt, n) \<in> set produced \<longrightarrow>
+      p = 1 \<and> n = 1 \<and> myfst pt \<in> set (timestamps os_label_prop_consumed) \<and> MyPair (myfst pt) 0 \<le> pt) \<and>
+    (\<forall>p pt n. (p, pt, n) \<in> set (
+        map (\<lambda>(x, cap). case cap of Cap t p \<Rightarrow> (p, t, 1))
+          (snd (label_prop_input1_batched os_label_prop_consumed (input os_label_prop_consumed 1)))) \<longrightarrow>
+      p = 1 \<and> n = 1 \<and> myfst pt \<in> set (timestamps os_label_prop_consumed) \<and> MyPair (myfst pt) 0 \<le> pt)\<close>
+proof -
+  obtain produced where prod_eq:
+    \<open>produ (fst (snd (loop_updates cbufs os_label_prop os))) =
+      produ os_label_prop @
+        map (\<lambda>(x, cap). case cap of Cap t p \<Rightarrow> (p, t, 1))
+          (snd (label_prop_input1_batched os_label_prop_consumed (input os_label_prop_consumed 1))) @
+        produced\<close>
+    and props: \<open>\<forall>p pt n. (p, pt, n) \<in> set (
+        map (\<lambda>(x, cap). case cap of Cap t p \<Rightarrow> (p, t, 1))
+          (snd (label_prop_input1_batched os_label_prop_consumed (input os_label_prop_consumed 1))) @ produced) \<longrightarrow>
+      p = 1 \<and> n = 1 \<and> myfst pt \<in> set (timestamps os_label_prop_consumed) \<and> MyPair (myfst pt) 0 \<le> pt\<close>
+    by (rule produ_fst_snd_loop_updatesE
+        [where os = os and os_label_prop = os_label_prop
+          and os_label_prop_consumed = os_label_prop_consumed and cbufs = cbufs,
+          OF INV LABELS TIMES os_label_prop_consumed_def])
+  show ?thesis
+    using prod_eq props 
+    by (smt (verit, del_insts) append.assoc in_set_conv_decomp label_prop_input1_batched_produced_memberD)
+qed
+
+
 
 
 
@@ -2751,6 +3102,20 @@ lemma extract_prog_three_fold:
    extract_progress 2 eds (snd (obtain_progress os2)) =
    extract_prog [0 :: 3, 1, 2] eds (\<lambda> nid. if nid = 0 then os0 else if nid = 1 then os1 else os2)\<close>
   by (simp add: extract_prog_def)
+lemma buff_sim_aux[simp]:
+  "(\<lambda>p'. if Inr (1, 0) = p'
+                    then drop (length (cbufs (1, 0)) -+- length (outpu (os 0) 0) -+- length (filter is_Data (ltaken n lxs)))
+                          (((\<lambda>p'a. if p' = p'a then map Inr (outpu (os 0) 0) @ map (\<lambda>ev. case ev of Data t d \<Rightarrow> Inr (Inl d, t)) (filter is_Data (ltaken n lxs)) else []) >>
+                            case_sum (\<lambda>x. []) (\<lambda>x. map Inr (cbufs x)))
+                            p')
+                    else ((\<lambda>p'. if Inr (1, 0) = p' then map Inr (outpu (os 0) 0) @ map (\<lambda>ev. case ev of Data t d \<Rightarrow> Inr (Inl d, t)) (filter is_Data (ltaken n lxs)) else []) >>
+                          case_sum (\<lambda>x. []) (\<lambda>x. map Inr (cbufs x)))
+                          p') = case_sum (\<lambda>x. []) (\<lambda>x. map Inr ((cbufs((1, 0) := [])) x))"
+  apply (rule ext)+
+  unfolding BULK_BENQ_def
+  apply (auto split: sum.splits)
+  done
+
 
 lemma label_propagation_correctness:
   fixes lxs :: \<open>((nat, nat) myprod, nat \<times> nat) event llist\<close>
@@ -2932,28 +3297,28 @@ proof (coinduction arbitrary: S SO SP D lxs os os_input os_label_prop cbufs chns
                             apply (rule refl)
         using subgraph_inv(1) apply simp
                             apply (simp_all add: operator_state.defs(3) subgraph_inv(2) os_inv)
-        apply (simp add: consumes_def add_caps_def BENQ_def)
-        apply (intro conjI)
-        apply (simp add: raw_summary_def fun_eq_iff)
-        apply (rule refl)
-        apply (rule refl)
-        apply (rule refl)
-        apply (rule refl)
+                     apply (simp add: consumes_def add_caps_def BENQ_def)
+                     apply (intro conjI)
+                         apply (simp add: raw_summary_def fun_eq_iff)
+                        apply (rule refl)
+                       apply (rule refl)
+                      apply (rule refl)
+                     apply (rule refl)
         using os_inv(1,5)
-        apply (simp add: ty1_check_def operator_state.defs(3) BTL_def)
-        apply blast
+                    apply (simp add: ty1_check_def operator_state.defs(3) BTL_def)
+                    apply blast
         using os_inv(1,4-6)
-        apply (simp add: ty1_check_def label_prob_ty2_check_def operator_state.defs(3) BTL_def BHD_def)
-        apply (erule conjE)
-        apply (rotate_tac 9)
-        apply (drule spec[of _ 0])
-        apply (simp add: Ball_def)
-        apply (meson img_fst in_fst_imageE in_set_tlD)
-        apply (rule dataplane_tracker_inv_consumes[OF dataplane_inv _ D G, where xs=\<open>tl (cbufs (1, p))\<close>])
-        apply (simp add: BHD_def)
-        apply (simp add: csets_inv(1) buffers_inv os_inv(4,7) operator_state.defs(3) consumes_def)
-        apply (simp add: csets_inv(2))
-        apply (rule input_stream_inv)
+                   apply (simp add: ty1_check_def label_prob_ty2_check_def operator_state.defs(3) BTL_def BHD_def)
+                   apply (erule conjE)
+                   apply (rotate_tac 9)
+                   apply (drule spec[of _ 0])
+                   apply (simp add: Ball_def)
+                   apply (meson img_fst in_fst_imageE in_set_tlD)
+                  apply (rule dataplane_tracker_inv_consumes[OF dataplane_inv _ D G, where xs=\<open>tl (cbufs (1, p))\<close>])
+                  apply (simp add: BHD_def)
+                 apply (simp add: csets_inv(1) buffers_inv os_inv(4,7) operator_state.defs(3) consumes_def)
+                apply (simp add: csets_inv(2))
+               apply (rule input_stream_inv)
         using label_prop_inv(1) apply (simp add: os_inv(4,7) operator_state.defs(3))
         using label_prop_inv(2) apply (simp add: os_inv(4,7) operator_state.defs(3) consumes_def)
         subgoal
@@ -2964,18 +3329,18 @@ proof (coinduction arbitrary: S SO SP D lxs os os_input os_label_prop cbufs chns
             using prems(2,10-12) prems(4)[symmetric] unfolding front_inv_def imp_front_inv_def chnls_imp_front_inv_def
             apply simp
             apply (rule contrapos_pp[OF _ frontier_less_equal_exit_scope, rotated, where t1=\<open>t -+- MyPair 0 1\<close>])
-            apply simp
+             apply simp
             apply (drule spec2[of _ 1 1])
             apply (drule spec[of _ \<open>Loc 1 (Trg 1)\<close>])
             apply (drule spec2[of _ 1 0])
             apply (drule bspec[of _ _ \<open>(d, t)\<close>])
-            apply (simp add: BULK_BENQ_def BHD_def)
-            apply (rule disjI1)
-            apply (metis list.set_sel(1))
+             apply (simp add: BULK_BENQ_def BHD_def)
+             apply (rule disjI1)
+             apply (metis list.set_sel(1))
             apply (rule frontier_less_equal_le_trans[rotated])
-            apply (rule order.trans)
-            apply assumption
-            apply assumption
+             apply (rule order.trans)
+              apply assumption
+             apply assumption
             apply (rule frontier_less_equal_ifrontier_trans[OF D, where l=\<open>Loc 1 (Trg 0)\<close>])
             using path_weight_loop_increment apply (simp add: subgraph_inv(1))
             apply simp
@@ -2985,25 +3350,25 @@ proof (coinduction arbitrary: S SO SP D lxs os os_input os_label_prop cbufs chns
           using prems(2) prems(4)[symmetric] buffers_inv label_prop_inv(4) hd_in_set
           by (fastforce simp add: raw_summary_def BULK_BENQ_def BHD_def)
         using label_prop_inv(5) apply (simp add: os_inv(4,7) operator_state.defs(3) consumes_def)
-        apply (subst label_prop_upd_inv_cong; simp add: BENQ_def)
-        apply (rule inputs_ocaps_inv_consumes[OF label_prop_inv(6)])
+          apply (subst label_prop_upd_inv_cong; simp add: BENQ_def)
+         apply (rule inputs_ocaps_inv_consumes[OF label_prop_inv(6)])
         apply (clarsimp simp add: dataflow_tree_to_operator_def intro!: arg_cong[where f=\<open>set_op _ _\<close>] arg_cong[where f=\<open>dataflow_op _\<close>] arg_cong[where f=\<open>map_op _ _\<close>])
         apply (rule arg_cong2[where f=\<open>\<lambda>buf op. comp_op _ buf _ op\<close>])
-        apply (simp add: BTL_def fun_eq_iff map_tl split: sum.splits)
+         apply (simp add: BTL_def fun_eq_iff map_tl split: sum.splits)
         apply (rule loop_op_buf_cong[OF refl])
-        apply (rule arg_cong[where f=\<open>map_op _ _\<close>])
-        apply (rule comp_op_buf_cong[OF refl refl refl])
-        apply (simp add: ran_comp_wire BTL_def)
+         apply (rule arg_cong[where f=\<open>map_op _ _\<close>])
+         apply (rule comp_op_buf_cong[OF refl refl refl])
+         apply (simp add: ran_comp_wire BTL_def)
         apply (simp add: ran_loop_wire BTL_def)
         done
       subgoal for os_input'
         apply (clarsimp simp add: ooo_input_op_logic_def split: llist.splits event.splits)
         subgoal
           apply (intro exI conjI relcomppI)
-          apply (rule rtranclp.rtrancl_refl)
-          apply (rule bisim_refl)
-          defer
-          apply (rule wbisim_refl)
+             apply (rule rtranclp.rtrancl_refl)
+            apply (rule bisim_refl)
+           defer
+           apply (rule wbisim_refl)
           apply (rule wb_upto_b_base)
           apply (unfold R_def)
           apply (rule exI)
@@ -3014,10 +3379,10 @@ proof (coinduction arbitrary: S SO SP D lxs os os_input os_label_prop cbufs chns
           apply (rule exI[of _ \<open>os(0 := drop_caps (os 0) (map (\<lambda>t. Cap t 0) (ocaps (os 0) 0)))\<close>])
           apply (rule exI[of _ os_input'])
           apply (intro exI conjI)
-          defer
-          apply (rule refl)
-          apply (rule subgraph_inv(1))
-          apply (rule subgraph_inv(2))
+                              defer
+                              apply (rule refl)
+                              apply (rule subgraph_inv(1))
+                              apply (rule subgraph_inv(2))
           using os_inv(1) apply (simp add: operator_state.defs(3) drop_caps_def)
           using os_inv(2) apply simp
           using os_inv(3) apply simp
@@ -3029,9 +3394,9 @@ proof (coinduction arbitrary: S SO SP D lxs os os_input os_label_prop cbufs chns
           using os_inv(9) apply simp
           using buffers_inv apply fast
           using dataplane_tracker_inv_drop_caps_all[OF D G subgraph_inv(2) dataplane_inv] apply blast
-          apply (simp add: csets_inv(1) buffers_inv os_inv(1,4) operator_state.defs(3))
-          apply (simp add: csets_inv(2))
-          apply (simp add: ocaps_drop_caps_all(1))
+                   apply (simp add: csets_inv(1) buffers_inv os_inv(1,4) operator_state.defs(3))
+                  apply (simp add: csets_inv(2))
+                 apply (simp add: ocaps_drop_caps_all(1))
           using label_prop_inv(1) os_inv(4) apply fast
           using label_prop_inv(2) os_inv(4) apply simp
           using label_prop_inv(3) apply simp
@@ -3042,10 +3407,10 @@ proof (coinduction arbitrary: S SO SP D lxs os os_input os_label_prop cbufs chns
           done
         subgoal for lxs' t v w
           apply (intro exI conjI relcomppI)
-          apply (rule rtranclp.rtrancl_refl)
-          apply (rule bisim_refl)
-          defer
-          apply (rule wbisim_refl)
+             apply (rule rtranclp.rtrancl_refl)
+            apply (rule bisim_refl)
+           defer
+           apply (rule wbisim_refl)
           apply (rule wb_upto_b_base)
           apply (unfold R_def)
           apply (rule exI)
@@ -3059,10 +3424,10 @@ proof (coinduction arbitrary: S SO SP D lxs os os_input os_label_prop cbufs chns
           apply (rule exI[of _ cbufs])
           apply (rule exI[of _ \<open>BENQ (1, 0) (en1 os_input (v, w), t) chns\<close>])
           apply (intro exI conjI)
-          defer
-          apply (rule refl)
-          apply (rule subgraph_inv(1))
-          apply (rule subgraph_inv(2))
+                              defer
+                              apply (rule refl)
+                              apply (rule subgraph_inv(1))
+                              apply (rule subgraph_inv(2))
           using os_inv(1) apply (simp add: produce_def operator_state.defs(3))
           using os_inv(2) apply (simp add: produce_def)
           using os_inv(3) apply (simp add: produce_def)
@@ -3073,12 +3438,12 @@ proof (coinduction arbitrary: S SO SP D lxs os os_input os_label_prop cbufs chns
 
           using os_inv(8) apply simp
           using os_inv(9) apply simp
-          apply (simp add: buffers_inv BENQ_def BULK_BENQ_def outputs_at_target_raw_summary subgraph_inv(1) inputs_at_target_def fun_eq_iff produce_def)
-          apply (rule dataplane_tracker_inv_produce_singleton[OF D G subgraph_inv(2) dataplane_inv, where t=t and nid=0 and p=0])
+                     apply (simp add: buffers_inv BENQ_def BULK_BENQ_def outputs_at_target_raw_summary subgraph_inv(1) inputs_at_target_def fun_eq_iff produce_def)
+                    apply (rule dataplane_tracker_inv_produce_singleton[OF D G subgraph_inv(2) dataplane_inv, where t=t and nid=0 and p=0])
           using input_stream_inv apply (fastforce simp add: timely_input_stream_def os_inv(1) operator_state.defs(3))
-          apply (rule refl)
-          apply (simp add: csets_inv(1) os_inv(1,4) operator_state.defs(3))
-          apply (simp add: csets_inv(2))
+                    apply (rule refl)
+                   apply (simp add: csets_inv(1) os_inv(1,4) operator_state.defs(3))
+                  apply (simp add: csets_inv(2))
           using input_stream_inv apply (fastforce simp add: os_inv(1) operator_state.defs(3) produce_def)
           using label_prop_inv(1) os_inv(4) apply fast
           using label_prop_inv(2) os_inv(4) apply simp
@@ -3090,10 +3455,10 @@ proof (coinduction arbitrary: S SO SP D lxs os os_input os_label_prop cbufs chns
           done
         subgoal for lxs' t
           apply (intro exI conjI relcomppI)
-          apply (rule rtranclp.rtrancl_refl)
-          apply (rule bisim_refl)
-          defer
-          apply (rule wbisim_refl)
+             apply (rule rtranclp.rtrancl_refl)
+            apply (rule bisim_refl)
+           defer
+           apply (rule wbisim_refl)
           apply (rule wb_upto_b_base)
           apply (unfold R_def)
           apply (rule exI)
@@ -3104,10 +3469,10 @@ proof (coinduction arbitrary: S SO SP D lxs os os_input os_label_prop cbufs chns
           apply (rule exI[of _ \<open>os(0 := drop_cap (os 0) (Cap t 0))\<close>])
           apply (rule exI[of _ os_input'])
           apply (intro exI conjI)
-          defer
-          apply (rule refl)
-          apply (rule subgraph_inv(1))
-          apply (rule subgraph_inv(2))
+                              defer
+                              apply (rule refl)
+                              apply (rule subgraph_inv(1))
+                              apply (rule subgraph_inv(2))
           using os_inv(1) apply (simp add: drop_cap_def operator_state.defs(3))
           using os_inv(2) apply (simp add: drop_cap_def)
           using os_inv(3) apply (simp add: drop_cap_def)
@@ -3117,16 +3482,16 @@ proof (coinduction arbitrary: S SO SP D lxs os os_input os_label_prop cbufs chns
           using os_inv(7) apply (simp add: drop_cap_def)
           using os_inv(8) apply simp
           using os_inv(9) apply simp
-          apply (simp add: buffers_inv)
-          apply (rule dataplane_tracker_inv_drop_cap[OF D G subgraph_inv(2) dataplane_inv, where t=t and nid=0 and p=0])
+                     apply (simp add: buffers_inv)
+                    apply (rule dataplane_tracker_inv_drop_cap[OF D G subgraph_inv(2) dataplane_inv, where t=t and nid=0 and p=0])
           using input_stream_inv apply (fastforce simp add: timely_input_stream_def os_inv(1) operator_state.defs(3))
-          apply (rule refl)
-          apply (simp add: csets_inv(1) os_inv(1,4) operator_state.defs(3) buffers_inv BULK_BENQ_def outputs_at_target_raw_summary subgraph_inv(1) inputs_at_target_def)
-          apply (subst (1 2) icoll_lshift)
+                    apply (rule refl)
+                   apply (simp add: csets_inv(1) os_inv(1,4) operator_state.defs(3) buffers_inv BULK_BENQ_def outputs_at_target_raw_summary subgraph_inv(1) inputs_at_target_def)
+                   apply (subst (1 2) icoll_lshift)
           using timely_input_stream_expires_le input_stream_inv apply blast
           using timely_input_stream_expires_le input_stream_inv apply blast
-          apply simp
-          apply (simp add: csets_inv(2))
+                   apply simp
+                  apply (simp add: csets_inv(2))
           using input_stream_inv apply (fastforce simp add: os_inv(1) operator_state.defs(3) drop_cap_def)
           using label_prop_inv(1) os_inv(4) apply fast
           using label_prop_inv(2) os_inv(4) apply simp
@@ -3138,10 +3503,10 @@ proof (coinduction arbitrary: S SO SP D lxs os os_input os_label_prop cbufs chns
           done
         subgoal for lxs' t
           apply (intro exI conjI relcomppI)
-          apply (rule rtranclp.rtrancl_refl)
-          apply (rule bisim_refl)
-          defer
-          apply (rule wbisim_refl)
+             apply (rule rtranclp.rtrancl_refl)
+            apply (rule bisim_refl)
+           defer
+           apply (rule wbisim_refl)
           apply (rule wb_upto_b_base)
           apply (unfold R_def)
           apply (rule exI)
@@ -3152,10 +3517,10 @@ proof (coinduction arbitrary: S SO SP D lxs os os_input os_label_prop cbufs chns
           apply (rule exI[of _ \<open>os(0 := add_cap (os 0) 0 t)\<close>])
           apply (rule exI[of _ os_input'])
           apply (intro exI conjI)
-          defer
-          apply (rule refl)
-          apply (rule subgraph_inv(1))
-          apply (rule subgraph_inv(2))
+                              defer
+                              apply (rule refl)
+                              apply (rule subgraph_inv(1))
+                              apply (rule subgraph_inv(2))
           using os_inv(1) apply (simp add: add_cap_def operator_state.defs(3))
           using os_inv(2) apply (simp add: add_cap_def)
           using os_inv(3) apply (simp add: add_cap_def)
@@ -3165,16 +3530,16 @@ proof (coinduction arbitrary: S SO SP D lxs os os_input os_label_prop cbufs chns
           using os_inv(7) apply (simp add: add_cap_def)
           using os_inv(8) apply simp
           using os_inv(9) apply simp
-          apply (simp add: buffers_inv)
-          apply (rule dataplane_tracker_inv_add_cap[OF D dataplane_inv G, where t=t and nid=0 and p=0])
+                     apply (simp add: buffers_inv)
+                    apply (rule dataplane_tracker_inv_add_cap[OF D dataplane_inv G, where t=t and nid=0 and p=0])
           using input_stream_inv apply (fastforce simp add: os_inv(1) operator_state.defs(3) timely_input_stream_def)
-          apply (rule refl)
-          apply (simp add: csets_inv(1) os_inv(1,4) operator_state.defs(3) buffers_inv BULK_BENQ_def outputs_at_target_raw_summary subgraph_inv(1) inputs_at_target_def)
-          apply (subst (1 2) icoll_lshift)
+                    apply (rule refl)
+                   apply (simp add: csets_inv(1) os_inv(1,4) operator_state.defs(3) buffers_inv BULK_BENQ_def outputs_at_target_raw_summary subgraph_inv(1) inputs_at_target_def)
+                   apply (subst (1 2) icoll_lshift)
           using timely_input_stream_expires_le input_stream_inv apply blast
           using timely_input_stream_expires_le input_stream_inv apply blast
-          apply (simp add: add_cap_def)
-          apply (simp add: csets_inv(2))
+                   apply (simp add: add_cap_def)
+                  apply (simp add: csets_inv(2))
           using input_stream_inv apply (force simp add: os_inv(1) operator_state.defs(3) add_cap_def)
           using label_prop_inv(1) os_inv(4) apply fast
           using label_prop_inv(2) os_inv(4) apply simp
@@ -3187,11 +3552,11 @@ proof (coinduction arbitrary: S SO SP D lxs os os_input os_label_prop cbufs chns
         done
       subgoal for d t xs
         apply (intro exI conjI)
-        apply (rule rtranclp.rtrancl_refl)
+         apply (rule rtranclp.rtrancl_refl)
         apply (intro relcomppI)
-        apply (rule bisim_refl)
-        defer
-        apply (rule wbisim_refl)
+          apply (rule bisim_refl)
+         defer
+         apply (rule wbisim_refl)
         apply (rule wb_upto_b_base)
         apply (unfold R_def[simplified])
         apply (rule exI[of _ S])
@@ -3202,34 +3567,34 @@ proof (coinduction arbitrary: S SO SP D lxs os os_input os_label_prop cbufs chns
         apply (rule exI[of _ \<open>BENQ (2, 1) (d, t) cbufs\<close>])
         apply (rule exI[of _ sg])
         apply (intro conjI)
-        apply (clarsimp simp add: dataflow_tree_to_operator_def os_inv(1)
+                           apply (clarsimp simp add: dataflow_tree_to_operator_def os_inv(1)
             intro!: arg_cong[where f=\<open>set_op _ _\<close>] arg_cong[where f=\<open>dataflow_op _\<close>]
             arg_cong[where f=\<open>map_op _ _\<close>])
-        apply (rule comp_op_buf_cong[OF refl refl])
-        apply (rule loop_op_buf_cong[OF refl])
-        apply (rule arg_cong[where f=\<open>map_op _ _\<close>])
-        apply (rule comp_op_buf_cong[OF refl refl refl])
-        apply (simp add: ran_comp_wire)
-        apply (simp add: ran_loop_wire BENQ_def)
-        apply (clarsimp simp add: BENQ_def ran_def split: sum.splits)
-        apply (metis obj_sumE prod.exhaust)
-        apply (simp add: cimage_cUn csets_inv buffers_inv outputs_at_target_raw_summary subgraph_inv(1) os_inv(1,4) operator_state.defs(3) BENQ_def BULK_BENQ_def all_edges_def all_vertices_def neighbors_def)
-        apply (rule subgraph_inv(1))
-        apply (rule subgraph_inv(2))
-        apply (simp add: os_inv(2))
-        apply (simp add: os_inv(3))
-        apply (simp add: os_inv(4) operator_state.defs(3))
+                           apply (rule comp_op_buf_cong[OF refl refl])
+                            apply (rule loop_op_buf_cong[OF refl])
+                            apply (rule arg_cong[where f=\<open>map_op _ _\<close>])
+                            apply (rule comp_op_buf_cong[OF refl refl refl])
+                            apply (simp add: ran_comp_wire)
+                            apply (simp add: ran_loop_wire BENQ_def)
+                           apply (clarsimp simp add: BENQ_def ran_def split: sum.splits)
+                           apply (metis obj_sumE prod.exhaust)
+                          apply (simp add: cimage_cUn csets_inv buffers_inv outputs_at_target_raw_summary subgraph_inv(1) os_inv(1,4) operator_state.defs(3) BENQ_def BULK_BENQ_def all_edges_def all_vertices_def neighbors_def)
+                         apply (rule subgraph_inv(1))
+                        apply (rule subgraph_inv(2))
+                       apply (simp add: os_inv(2))
+                      apply (simp add: os_inv(3))
+                     apply (simp add: os_inv(4) operator_state.defs(3))
         using os_inv(1,5) apply (simp add: BENQ_def ty1_check_def)
         using os_inv(6) apply (simp add: BENQ_def label_prob_ty2_check_def)
         using os_inv(7) apply simp
         using os_inv(8) apply simp
         using os_inv(9) apply simp
-        apply (rule dataplane_tracker_inv_update_outputs[OF dataplane_inv _ _ _ _ G, where nid=1 and p=1 and xs=\<open>[(d, t)]\<close>])
-        apply (simp add: os_inv(4) operator_state.defs(3))
-        apply (simp add: fun_upd_def)
-        apply (simp add: BENQ_def)
-        apply (simp add: subgraph_inv(1) raw_summary_def antichain_from_list_singleton)
-        apply (simp add: input_stream_inv)
+               apply (rule dataplane_tracker_inv_update_outputs[OF dataplane_inv _ _ _ _ G, where nid=1 and p=1 and xs=\<open>[(d, t)]\<close>])
+                  apply (simp add: os_inv(4) operator_state.defs(3))
+                 apply (simp add: fun_upd_def)
+                apply (simp add: BENQ_def)
+               apply (simp add: subgraph_inv(1) raw_summary_def antichain_from_list_singleton)
+              apply (simp add: input_stream_inv)
         subgoal
           using label_prop_inv
           by (simp add: all_edges_def all_vertices_def min_label_def neighbors_def labels_inv_def labels_stable_def)
@@ -3254,10 +3619,10 @@ proof (coinduction arbitrary: S SO SP D lxs os os_input os_label_prop cbufs chns
         done
       subgoal for d t
         apply (intro exI conjI relcomppI)
-        apply (rule rtranclp.rtrancl_refl)
-        apply (rule bisim_refl)
-        defer
-        apply (rule wbisim_refl)
+           apply (rule rtranclp.rtrancl_refl)
+          apply (rule bisim_refl)
+         defer
+         apply (rule wbisim_refl)
         apply (rule wb_upto_b_base)
         apply (unfold R_def[simplified])
         apply (rule exI[of _ S])
@@ -3268,20 +3633,20 @@ proof (coinduction arbitrary: S SO SP D lxs os os_input os_label_prop cbufs chns
         apply (rule exI[of _ \<open>BTL (2, 1) cbufs\<close>])
         apply (rule exI[of _ sg])
         apply (intro conjI)
-        apply (clarsimp simp add: dataflow_tree_to_operator_def os_inv(1)
+                           apply (clarsimp simp add: dataflow_tree_to_operator_def os_inv(1)
             intro!: arg_cong[where f=\<open>set_op _ _\<close>] arg_cong[where f=\<open>dataflow_op _\<close>]
             arg_cong[where f=\<open>map_op _ _\<close>])
-        apply (rule comp_op_buf_cong[OF refl refl])
-        apply (rule loop_op_buf_cong[OF refl])
-        apply (rule arg_cong[where f=\<open>map_op _ _\<close>])
-        apply (rule comp_op_buf_cong[OF refl refl refl])
-        apply (simp add: ran_comp_wire BTL_def map_tl)
-        apply (simp add: ran_loop_wire BTL_def)
-        apply (simp add: BTL_def ran_def split: sum.splits)
-        apply (metis prod.exhaust sum.exhaust)
-        apply (simp add: csets_inv buffers_inv BULK_BENQ_def BENQ_def BTL_def cimage_cUn)
-        apply (rule subgraph_inv(1))
-        apply (rule subgraph_inv(2))
+                           apply (rule comp_op_buf_cong[OF refl refl])
+                            apply (rule loop_op_buf_cong[OF refl])
+                            apply (rule arg_cong[where f=\<open>map_op _ _\<close>])
+                            apply (rule comp_op_buf_cong[OF refl refl refl])
+                            apply (simp add: ran_comp_wire BTL_def map_tl)
+                            apply (simp add: ran_loop_wire BTL_def)
+                           apply (simp add: BTL_def ran_def split: sum.splits)
+                           apply (metis prod.exhaust sum.exhaust)
+                          apply (simp add: csets_inv buffers_inv BULK_BENQ_def BENQ_def BTL_def cimage_cUn)
+                         apply (rule subgraph_inv(1))
+                        apply (rule subgraph_inv(2))
         using os_inv(2) apply simp
         using os_inv(3) apply simp
         using os_inv(4) apply force
@@ -3290,29 +3655,29 @@ proof (coinduction arbitrary: S SO SP D lxs os os_input os_label_prop cbufs chns
         using os_inv(7) apply force
         using os_inv(8) apply (simp add: inputs_ocaps_inv_consumes)
         using os_inv(9) apply simp
-        apply (rule dataplane_tracker_inv_consumes[OF dataplane_inv _ D G, where xs=\<open>tl (cbufs (2, 1))\<close>])
-        apply (simp add: BHD_def)
+               apply (rule dataplane_tracker_inv_consumes[OF dataplane_inv _ D G, where xs=\<open>tl (cbufs (2, 1))\<close>])
+               apply (simp add: BHD_def)
         using input_stream_inv apply simp
         using label_prop_inv(1) apply (simp add: os_inv(4,7) operator_state.defs(3))
         using label_prop_inv(2) apply (simp add: os_inv(4,7) operator_state.defs(3) consumes_def)
         using label_prop_inv(3) apply simp
         using label_prop_inv(4) apply (simp add: buffers_inv BULK_BENQ_def BTL_def BENQ_def)
-        apply (rule label_prop_inv(5))
+         apply (rule label_prop_inv(5))
         using label_prop_inv(6) apply simp
         done
       subgoal for os'
         unfolding label_propagation_op_logic_def trace_simp
         apply clarsimp
         apply (elim disjE)
-        prefer 3
+          prefer 3
         subgoal
           apply (simp split: if_splits prod.splits)
           apply hypsubst_thin
           apply (intro exI conjI relcomppI)
-          apply (rule rtranclp.intros(1))
-          apply (rule bisim_refl)
-          defer
-          apply (rule wbisim_refl)
+             apply (rule rtranclp.intros(1))
+            apply (rule bisim_refl)
+           defer
+           apply (rule wbisim_refl)
           apply (rule wb_upto_b_base)
           unfolding R_def[simplified]
           apply (rule exI[of _ S])
@@ -3335,10 +3700,10 @@ proof (coinduction arbitrary: S SO SP D lxs os os_input os_label_prop cbufs chns
             by (simp add: dataflow_tree_to_operator_def os_inv(1))
           subgoal premises aux
             apply (rule arg_cong2[where f=set_spec_op])
-            apply (simp_all add: subgraph_inv(1) buffers_inv csets_inv(1,2) outputs_at_target_raw_summary BULK_BENQ_def flip: list_diff_append map_append filter_append)
+             apply (simp_all add: subgraph_inv(1) buffers_inv csets_inv(1,2) outputs_at_target_raw_summary BULK_BENQ_def flip: list_diff_append map_append filter_append)
             apply (simp only: cUn_assoc)
             apply (rule arg_cong2[where f=cUn])
-            apply simp
+             apply simp
             apply (subst cset_eq_iff)
             apply (intro allI iffI)
             subgoal for x
@@ -3389,7 +3754,7 @@ proof (coinduction arbitrary: S SO SP D lxs os os_input os_label_prop cbufs chns
                       apply (subgoal_tac "myfst t' |\<in>| cset_from_list T ")
                       subgoal
                         apply (rule cBexI[rotated])
-                        apply assumption
+                         apply assumption
                         apply simp
                         apply (subgoal_tac "filter (\<lambda>y. y \<le> myfst t') T \<noteq> []")
                         subgoal
@@ -3416,7 +3781,7 @@ proof (coinduction arbitrary: S SO SP D lxs os os_input os_label_prop cbufs chns
                                 unfolding icoll_def
                                 apply simp
                                 apply (subst lfilter_False)
-                                apply simp_all
+                                 apply simp_all
                                 apply (clarsimp split: event.splits)
                                 apply (metis (no_types, opaque_lifting) MyPair_mono dataflow_topology_from_tree.zero_le dual_order.eq_iff event.discI(1) event.sel(1) frontier_less_equal_trans myprod.exhaust myprod.sel(1))
                                 done
@@ -3424,7 +3789,7 @@ proof (coinduction arbitrary: S SO SP D lxs os os_input os_label_prop cbufs chns
                                 apply safe
                                 subgoal for x
                                   apply (drule timely_input_stream_frontier_less_equal[OF input_stream_inv, rule_format, of x])
-                                  apply assumption
+                                   apply assumption
                                   using dataplane_inv[unfolded dataplane_tracker_inv_def, simplified, rule_format] apply -
                                   apply clarsimp
                                   unfolding front_inv_def imp_front_inv_def
@@ -3432,9 +3797,9 @@ proof (coinduction arbitrary: S SO SP D lxs os os_input os_label_prop cbufs chns
                                   apply (drule spec[of _ 0])
                                   apply (drule spec[of _ "Loc 1 (Trg 0)"])
                                   apply (rule frontier_less_equal_le_trans[rotated])
-                                  apply (rule order.trans)
-                                  apply assumption
-                                  apply assumption
+                                   apply (rule order.trans)
+                                    apply assumption
+                                   apply assumption
                                   subgoal for caps
                                     unfolding Src_caps_inv_def
                                     apply (drule spec[of _ 0])
@@ -3465,7 +3830,7 @@ proof (coinduction arbitrary: S SO SP D lxs os os_input os_label_prop cbufs chns
                             done
                           subgoal
                             apply (subgoal_tac "\<forall> t \<in> snd ` set ((outputs_at_target (summ sg) os >> cbufs) (1, 0)). frontier_less_equal (front (os 1) 0) t")
-                            defer
+                             defer
                             subgoal
                               apply safe
                               subgoal for _ a t
@@ -3483,8 +3848,8 @@ proof (coinduction arbitrary: S SO SP D lxs os os_input os_label_prop cbufs chns
                                 subgoal 
                                   by blast
                                 apply (drule frontier_less_equal_le_trans)
-                                apply (rule order.trans[rotated])
-                                apply assumption+
+                                 apply (rule order.trans[rotated])
+                                  apply assumption+
                                 done
                               done
                             subgoal
@@ -3500,7 +3865,7 @@ proof (coinduction arbitrary: S SO SP D lxs os os_input os_label_prop cbufs chns
                                   subgoal
                                     apply clarsimp
                                     apply (drule bspec, simp)
-                                    apply simp
+                                     apply simp
                                     subgoal for a b
                                       apply (cases b; cases t'; simp; hypsubst_thin?)
                                       subgoal for t1 t2 t3
@@ -3610,30 +3975,30 @@ proof (coinduction arbitrary: S SO SP D lxs os os_input os_label_prop cbufs chns
           using os_inv(9) apply simp
           subgoal premises aux
             apply (rule iffD1[OF dataplane_tracker_inv_clean, rotated 2, of _ _ sg "upfro sg"])
-            apply (rule dataplane_tracker_inv_produces_drops[OF D, where nid=1 and os=os 
+              apply (rule dataplane_tracker_inv_produces_drops[OF D, where nid=1 and os=os 
                   and drops = "\<lambda> p. if p = 1
                          then []
                          else filter (\<lambda>t. \<not> frontier_less_equal (exit_scope myfst (front os_label_prop 0 + front os_label_prop 1)) (myfst t) \<and> myfst t \<in> set (timestamps os_label_prop)) (ocaps os_label_prop 0)"
                   and produs="map (\<lambda> t . (0, MyPair t 0, 1)) (rmdups {} (map myfst (filter (\<lambda>t. \<not> frontier_less_equal (exit_scope myfst (front os_label_prop 0 + front os_label_prop 1)) (myfst t) \<and> myfst t \<in> set (timestamps os_label_prop)) (ocaps os_label_prop 0))))"
                   and oputs="(\<lambda> p. if p = 1 then [] else map (\<lambda>t. (en2 os_label_prop (components_from_labels (all_edges os_label_prop t) (min_label os_label_prop t)), (MyPair t 0)))
                           (rmdups {} (map myfst (filter (\<lambda>t. \<not> frontier_less_equal (exit_scope myfst (front os_label_prop 0 + front os_label_prop 1)) (myfst t) \<and> myfst t \<in> set (timestamps os_label_prop)) (ocaps os_label_prop 0)))))"])
-            apply (rule refl)+
-            prefer 9
+                         apply (rule refl)+
+                    prefer 9
             subgoal
               apply (intro allI impI conjI)
-              apply simp
+                     apply simp
               subgoal
                 apply (rule ext)+
                 unfolding produces_def drop_caps_def
                 apply auto
                 subgoal
                   apply (subst filter_False)
-                  apply auto
+                   apply auto
                   done
                 subgoal for p
                   apply (subst (2) filter_True)
-                  apply clarsimp
-                  apply (metis num2_neq(2))
+                   apply clarsimp
+                   apply (metis num2_neq(2))
                   apply (simp add: comp_def)
                   done
                 done
@@ -3650,7 +4015,7 @@ proof (coinduction arbitrary: S SO SP D lxs os os_input os_label_prop cbufs chns
                 unfolding produces_def drop_caps_def
                 apply (auto simp add: filter_True)
                 apply (subst filter_True)
-                apply auto
+                 apply auto
                 subgoal for p a t
                   apply (subgoal_tac "p = 0")
                   subgoal
@@ -3745,17 +4110,17 @@ proof (coinduction arbitrary: S SO SP D lxs os os_input os_label_prop cbufs chns
               apply (drule spec2[of _  0 1])
               apply simp
               apply (drule bspec[of _ ])
-              apply assumption
+               apply assumption
               apply (simp add: filter_True comp_def )
               done
             subgoal for a b
               apply (drule spec2[of _  0 0])
               apply simp
               apply (drule bspec[of _ ])
-              apply assumption
+               apply assumption
               apply (simp add: filter_True comp_def )
               apply (rule in_set_list_diffI)
-              apply fastforce
+               apply fastforce
               apply simp
               using label_prop_inv(3)[rule_format, of "myfst b"] apply -
               apply (drule meta_mp)
@@ -3770,10 +4135,10 @@ proof (coinduction arbitrary: S SO SP D lxs os os_input os_label_prop cbufs chns
               apply (drule spec2[of _  0 0])
               apply simp
               apply (drule bspec[of _ ])
-              apply assumption
+               apply assumption
               apply (simp add: filter_True comp_def )
               apply (rule in_set_list_diffI)
-              apply fastforce
+               apply fastforce
               apply simp
               using label_prop_inv(3)[rule_format, of "myfst b"] apply -
               apply (drule meta_mp)
@@ -3796,10 +4161,10 @@ proof (coinduction arbitrary: S SO SP D lxs os os_input os_label_prop cbufs chns
               subgoal for v1 v2 l1 l2
                 apply hypsubst_thin
                 apply (intro exI conjI relcomppI)
-                apply (rule rtranclp.intros(1))
-                apply (rule bisim_refl)
-                defer
-                apply (rule wbisim_refl)
+                   apply (rule rtranclp.intros(1))
+                  apply (rule bisim_refl)
+                 defer
+                 apply (rule wbisim_refl)
                 apply (rule wb_upto_b_base)
                 unfolding R_def[simplified]
                 apply (rule exI[of _ S])
@@ -3840,7 +4205,7 @@ proof (coinduction arbitrary: S SO SP D lxs os os_input os_label_prop cbufs chns
                   using aux(1,2,3) apply -
                   apply (simp  del: filter.simps add: label_prop_edge_batch_def label_prop_edge_record_update_def buffers_inv operator_state.defs os_inv(4) csets_inv(1))
                   apply (rule arg_cong2[where f=set_spec_op])
-                  apply (simp_all del: filter.simps)
+                   apply (simp_all del: filter.simps)
                   apply (clarsimp simp del: filter.simps del: disjCI simp add: inputs_at_target_def BULK_BENQ_def operator_state.defs outputs_at_target_raw_summary subgraph_inv buffers_inv csets_inv(1) os_inv(4))
                   subgoal
                     apply (subst (1) icoll_LCons_Data)
@@ -3877,7 +4242,7 @@ proof (coinduction arbitrary: S SO SP D lxs os os_input os_label_prop cbufs chns
                                 apply (subst (3) cimage_cUn)
                                 apply (subst (2) cUn_assoc)
                                 apply (rule arg_cong2[where f=cUn])
-                                apply (simp add:  csets_inv(2))
+                                 apply (simp add:  csets_inv(2))
                                 apply (subst (1) cfilter_False)
                                 subgoal
                                   unfolding label_prop_neighbor_batch_def
@@ -3920,7 +4285,7 @@ proof (coinduction arbitrary: S SO SP D lxs os os_input os_label_prop cbufs chns
                       subgoal
                         using label_prop_inv(4)[rule_format, of t] apply -
                         apply (drule meta_mp)
-                        apply (simp add: buffers_inv BULK_BENQ_def inputs_at_target_def)
+                         apply (simp add: buffers_inv BULK_BENQ_def inputs_at_target_def)
                         subgoal
                           apply (cases t)
                           apply auto
@@ -3972,7 +4337,7 @@ proof (coinduction arbitrary: S SO SP D lxs os os_input os_label_prop cbufs chns
                 using os_inv(9) apply simp
                 subgoal premises aux
                   apply (rule dataplane_tracker_inv_release_caps_update[OF D])
-                  apply (rule dataplane_tracker_inv_add_caps_produces_drop_caps_update[OF D])
+                    apply (rule dataplane_tracker_inv_add_caps_produces_drop_caps_update[OF D])
                   using dataplane_inv apply simp
                   using G apply simp
                   using subgraph_inv(2) apply assumption 
@@ -3982,7 +4347,7 @@ proof (coinduction arbitrary: S SO SP D lxs os os_input os_label_prop cbufs chns
                       unfolding label_prop_edge_batch_def label_prop_neighbor_batch_def label_prop_edge_record_update_def
                       apply (auto del: disjCI simp add: image_iff split_beta)
                       apply (rule bexI[rotated])
-                      apply assumption
+                       apply assumption
                       apply (simp add: less_eq_myprod_def)
                       done
                     subgoal
@@ -4011,13 +4376,13 @@ proof (coinduction arbitrary: S SO SP D lxs os os_input os_label_prop cbufs chns
                       using label_prop_inv(5) by assumption
                     subgoal
                       by (clarsimp simp add: input_tl_def label_prop_edge_batch_def label_prop_neighbor_batch_def operator_state.defs os_inv(4) release_caps_def drop_caps_def produces_def)
-                    apply (clarsimp simp add: label_prop_edge_record_update_def input_tl_def label_prop_edge_batch_def label_prop_neighbor_batch_def operator_state.defs os_inv(4) release_caps_def drop_caps_def produces_def)
-                    apply simp
-                    apply (clarsimp simp add: label_prop_edge_record_update_def input_tl_def label_prop_edge_batch_def label_prop_neighbor_batch_def operator_state.defs os_inv(4) release_caps_def drop_caps_def produces_def)
-                    apply simp
-                    apply (clarsimp simp add: label_prop_edge_record_update_def input_tl_def label_prop_edge_batch_def label_prop_neighbor_batch_def operator_state.defs os_inv(4) release_caps_def drop_caps_def produces_def)
-                    apply (clarsimp simp add: label_prop_edge_record_update_def input_tl_def label_prop_edge_batch_def label_prop_neighbor_batch_def operator_state.defs os_inv(4) release_caps_def drop_caps_def produces_def)
-                    apply simp
+                        apply (clarsimp simp add: label_prop_edge_record_update_def input_tl_def label_prop_edge_batch_def label_prop_neighbor_batch_def operator_state.defs os_inv(4) release_caps_def drop_caps_def produces_def)
+                        apply simp
+                       apply (clarsimp simp add: label_prop_edge_record_update_def input_tl_def label_prop_edge_batch_def label_prop_neighbor_batch_def operator_state.defs os_inv(4) release_caps_def drop_caps_def produces_def)
+                       apply simp
+                      apply (clarsimp simp add: label_prop_edge_record_update_def input_tl_def label_prop_edge_batch_def label_prop_neighbor_batch_def operator_state.defs os_inv(4) release_caps_def drop_caps_def produces_def)
+                     apply (clarsimp simp add: label_prop_edge_record_update_def input_tl_def label_prop_edge_batch_def label_prop_neighbor_batch_def operator_state.defs os_inv(4) release_caps_def drop_caps_def produces_def)
+                     apply simp
                     apply (clarsimp simp add: label_prop_edge_record_update_def input_tl_def label_prop_edge_batch_def label_prop_neighbor_batch_def operator_state.defs os_inv(4) release_caps_def drop_caps_def produces_def)
                     done
                   done
@@ -4039,9 +4404,9 @@ proof (coinduction arbitrary: S SO SP D lxs os os_input os_label_prop cbufs chns
                       apply (subgoal_tac "\<not> myfst t \<le> t'")
                       subgoal
                         apply (rule labels_stable_input0_preserved)
-                        apply (rule label_prop_inv(2)[unfolded os_inv(4) operator_state.defs, simplified, rule_format, of t'])
-                        apply (simp add: os_inv(4) operator_state.defs)
-                        apply assumption+
+                              apply (rule label_prop_inv(2)[unfolded os_inv(4) operator_state.defs, simplified, rule_format, of t'])
+                               apply (simp add: os_inv(4) operator_state.defs)
+                              apply assumption+
                         using aux[unfolded os_inv(4) operator_state.defs, simplified] apply (auto simp add: label_prop_edge_record_update_def  os_inv(4) operator_state.defs)
                         done
                       subgoal
@@ -4064,8 +4429,8 @@ proof (coinduction arbitrary: S SO SP D lxs os os_input os_label_prop cbufs chns
                   by (auto simp add: buffers_inv BULK_BENQ_def outputs_at_target_raw_summary subgraph_inv(1) inputs_at_target_def input_tl_def release_caps_def drop_caps_def add_caps_def label_prop_edge_record_update_def label_prop_edge_batch_def label_prop_neighbor_batch_def dest!: in_set_list_diffD in_set_tlD)
                 subgoal
                   apply (rule label_prop_upd_inv_input0_preserved)
-                  apply (rule label_prop_inv(5))
-                  apply (simp_all add: operator_state.defs os_inv(4))
+                         apply (rule label_prop_inv(5))
+                        apply (simp_all add: operator_state.defs os_inv(4))
                   unfolding label_prop_edge_record_update_def input_tl_def label_prop_edge_batch_def label_prop_neighbor_batch_def release_caps_def drop_caps_def add_caps_def
                   by (auto simp add: operator_state.defs os_inv(4)  input_tl_def release_caps_def drop_caps_def produces_def)
                 subgoal premises aux
@@ -4088,10 +4453,10 @@ proof (coinduction arbitrary: S SO SP D lxs os os_input os_label_prop cbufs chns
               subgoal for v l
                 apply hypsubst_thin
                 apply (intro exI conjI relcomppI)
-                apply (rule rtranclp.intros(1))
-                apply (rule bisim_refl)
-                defer
-                apply (rule wbisim_refl)
+                   apply (rule rtranclp.intros(1))
+                  apply (rule bisim_refl)
+                 defer
+                 apply (rule wbisim_refl)
                 apply (rule wb_upto_b_base)
                 unfolding R_def[simplified]
                 apply (rule exI[of _ S])
@@ -4124,7 +4489,7 @@ proof (coinduction arbitrary: S SO SP D lxs os os_input os_label_prop cbufs chns
                   using aux(2,3) apply -
                   apply (simp  del: filter.simps add: label_prop_edge_batch_def label_prop_edge_record_update_def buffers_inv operator_state.defs os_inv(4) csets_inv(1))
                   apply (rule arg_cong2[where f=set_spec_op])
-                  apply (clarsimp simp del: filter.simps del: disjCI simp add: inputs_at_target_def BULK_BENQ_def operator_state.defs outputs_at_target_raw_summary subgraph_inv buffers_inv csets_inv(1) os_inv(4))
+                   apply (clarsimp simp del: filter.simps del: disjCI simp add: inputs_at_target_def BULK_BENQ_def operator_state.defs outputs_at_target_raw_summary subgraph_inv buffers_inv csets_inv(1) os_inv(4))
                   subgoal
                     apply (simp add: cUn_assoc)
                     apply (rule arg_cong2[where f=cUn])
@@ -4182,9 +4547,9 @@ proof (coinduction arbitrary: S SO SP D lxs os os_input os_label_prop cbufs chns
                   using os_inv(2,4,6) apply -
                   apply simp
                   apply (rule label_prob_ty2_check_producesI)
-                  apply simp
-                  apply (rule label_prob_ty2_check_input_tlI)
-                  apply (auto simp add: operator_state.defs label_prop_label_batch_def label_prop_neighbor_batch_def)
+                    apply simp
+                    apply (rule label_prob_ty2_check_input_tlI)
+                    apply (auto simp add: operator_state.defs label_prop_label_batch_def label_prop_neighbor_batch_def)
                   done
                 subgoal
                   using os_inv(7) by simp
@@ -4192,7 +4557,7 @@ proof (coinduction arbitrary: S SO SP D lxs os os_input os_label_prop cbufs chns
                 using os_inv(9) apply simp
                 subgoal
                   apply (rule dataplane_tracker_inv_release_caps_update[OF D])
-                  apply (rule dataplane_tracker_inv_add_caps_produces_drop_caps_update[OF D])
+                    apply (rule dataplane_tracker_inv_add_caps_produces_drop_caps_update[OF D])
                   subgoal
                     using dataplane_inv by simp
                   subgoal
@@ -4221,9 +4586,9 @@ proof (coinduction arbitrary: S SO SP D lxs os os_input os_label_prop cbufs chns
                           of os_label_prop d t v l "myfst t"
                           "label_prop_label_record_update (input_tl os_label_prop 1) (myfst t) v (min (min_label os_label_prop (myfst t) v) l)" ta,
                           simplified])
-                    apply (rule label_prop_inv(1)[rule_format])
-                    apply (rule label_prop_inv(5))
-                    apply simp_all
+                       apply (rule label_prop_inv(1)[rule_format])
+                      apply (rule label_prop_inv(5))
+                     apply simp_all
                     done
                   done
                 subgoal
@@ -4250,8 +4615,8 @@ proof (coinduction arbitrary: S SO SP D lxs os os_input os_label_prop cbufs chns
                 subgoal
                   apply simp
                   apply (rule label_prop_upd_inv_input1_preserved[])
-                  apply (rule label_prop_inv(5))
-                  apply (simp_all add: label_prop_label_record_update_def input_tl_def image_iff os_inv(4) operator_state.defs)
+                           apply (rule label_prop_inv(5))
+                          apply (simp_all add: label_prop_label_record_update_def input_tl_def image_iff os_inv(4) operator_state.defs)
                   done
                 subgoal
                   apply simp
@@ -4269,10 +4634,10 @@ proof (coinduction arbitrary: S SO SP D lxs os os_input os_label_prop cbufs chns
       subgoal for os_incr'
         apply (clarsimp simp add: increment_op_logic_def if_splits)
         apply (intro exI conjI relcomppI)
-        apply (rule rtranclp.rtrancl_refl)
-        apply (rule bisim_refl)
-        defer
-        apply (rule wbisim_refl)
+           apply (rule rtranclp.rtrancl_refl)
+          apply (rule bisim_refl)
+         defer
+         apply (rule wbisim_refl)
         apply (rule wb_upto_b_base)
         apply (unfold R_def[simplified])
         apply (rule exI[of _ S])
@@ -4283,15 +4648,15 @@ proof (coinduction arbitrary: S SO SP D lxs os os_input os_label_prop cbufs chns
         apply (rule exI[of _ cbufs])
         apply (rule exI[of _ sg])
         apply (intro conjI)
-        apply (simp add: dataflow_tree_to_operator_def os_inv(1))
-        apply (simp add: csets_inv buffers_inv BULK_BENQ_def outputs_at_target_raw_summary subgraph_inv(1) inputs_at_target_def cimage_cUn)
-        apply (rule subgraph_inv(1))
-        apply (rule subgraph_inv(2))
+                           apply (simp add: dataflow_tree_to_operator_def os_inv(1))
+                          apply (simp add: csets_inv buffers_inv BULK_BENQ_def outputs_at_target_raw_summary subgraph_inv(1) inputs_at_target_def cimage_cUn)
+                         apply (rule subgraph_inv(1))
+                        apply (rule subgraph_inv(2))
         using os_inv(2) apply simp
         using os_inv(3) apply simp
         using os_inv(4) apply force
         using os_inv(1,5) apply simp
-        apply (rule os_inv(6))
+                   apply (rule os_inv(6))
         using os_inv(7) apply force
         using os_inv(7,8) apply (clarsimp simp add: input_ocaps_inv_def drop_caps_def produces_def raw_summary_def filter_False)
         using os_inv(9) apply simp
@@ -4301,17 +4666,17 @@ proof (coinduction arbitrary: S SO SP D lxs os os_input os_label_prop cbufs chns
                 and oputs=\<open>(\<lambda>_. [])(1 := map (\<lambda>(d, t). (d, t + MyPair 0 1)) (input (os 2) 1))\<close>]
           apply -
           apply (drule meta_mp)
-          apply simp
+           apply simp
           apply (drule meta_mp)
           using os_inv(7,8) apply (clarsimp simp add: split_beta input_ocaps_inv_def raw_summary_def)
           apply (drule meta_mp)
           using os_inv(7,8) apply (fastforce simp add: split_beta input_ocaps_inv_def raw_summary_def)
 
           apply (drule meta_mp)
-          apply (clarsimp simp add: comp_def split_beta filter_True filter_False)
+           apply (clarsimp simp add: comp_def split_beta filter_True filter_False)
           apply (subst dataplane_tracker_inv_clean_input)
-          defer
-          apply assumption
+           defer
+           apply assumption
           apply (clarsimp simp add: drop_caps_def produces_def comp_def split_beta fun_eq_iff)
           apply (rule conjI; clarsimp)
           subgoal for p
@@ -4320,11 +4685,11 @@ proof (coinduction arbitrary: S SO SP D lxs os os_input os_label_prop cbufs chns
             by (cases \<open>p = 1\<close>; clarsimp simp add: filter_True filter_False)
           done
         using input_stream_inv apply simp
-        apply (rule label_prop_inv(1))
+             apply (rule label_prop_inv(1))
         using label_prop_inv(2) apply simp
         using label_prop_inv(3) apply simp
         using label_prop_inv(4) apply (simp add: buffers_inv BULK_BENQ_def outputs_at_target_raw_summary subgraph_inv(1) inputs_at_target_def)
-        apply (rule label_prop_inv(5))
+         apply (rule label_prop_inv(5))
         using label_prop_inv(6) apply simp
         done
       subgoal 
@@ -4348,11 +4713,11 @@ proof (coinduction arbitrary: S SO SP D lxs os os_input os_label_prop cbufs chns
         sorry
       subgoal for d t xs
         apply (intro exI conjI)
-        apply (rule rtranclp.rtrancl_refl)
+         apply (rule rtranclp.rtrancl_refl)
         apply (intro relcomppI)
-        apply (rule bisim_refl)
-        defer
-        apply (rule wbisim_refl)
+          apply (rule bisim_refl)
+         defer
+         apply (rule wbisim_refl)
         apply (rule wb_upto_b_base)
         apply (unfold R_def[simplified])
         apply (rule exI[of _ \<open>cinsert ((1, 0), d, t) S\<close>])
@@ -4363,14 +4728,14 @@ proof (coinduction arbitrary: S SO SP D lxs os os_input os_label_prop cbufs chns
         apply (rule exI[of _ cbufs])
         apply (rule exI[of _ sg])
         apply (intro exI conjI)
-        apply (simp add: dataflow_tree_to_operator_def os_inv(1))
+                           apply (simp add: dataflow_tree_to_operator_def os_inv(1))
         subgoal
           apply (simp add: subgraph_inv outputs_at_target_raw_summary csets_inv(1,2) buffers_inv os_inv(4) operator_state.defs(3))
           apply (rule arg_cong2[where f=set_spec_op])
-          apply (rule arg_cong2[where f=cinsert])
-          apply simp_all
+           apply (rule arg_cong2[where f=cinsert])
+            apply simp_all
           apply (rule arg_cong2[where f=cUn])
-          apply simp
+           apply simp
           apply (rule cimage_cong)
           subgoal
             by simp
@@ -4378,25 +4743,25 @@ proof (coinduction arbitrary: S SO SP D lxs os os_input os_label_prop cbufs chns
             unfolding all_edges_def all_vertices_def set_neighbors
             by simp
           done
-        apply (rule subgraph_inv(1))
-        apply (rule subgraph_inv(2))
-        apply (simp add: os_inv(2))
-        apply (simp add: os_inv(3))
-        apply (simp add: os_inv(4) operator_state.defs(3))
+                         apply (rule subgraph_inv(1))
+                        apply (rule subgraph_inv(2))
+                       apply (simp add: os_inv(2))
+                      apply (simp add: os_inv(3))
+                     apply (simp add: os_inv(4) operator_state.defs(3))
         using os_inv(1,5) apply simp
         using os_inv(6) unfolding label_prob_ty2_check_def apply simp
         using os_inv(7) apply simp
         using os_inv(8) apply simp
         using os_inv(9) apply simp
-        apply (rule dataplane_tracker_inv_update_outputs_outside[OF dataplane_inv _ _ G])
-        apply (simp add: fun_upd_def)
-        apply (simp add: subgraph_inv(1) raw_summary_def)
-        apply (subgoal_tac \<open>outputs_at_target (summ sg) (os(1 := (os 1)\<lparr>outpu := (outpu (os 1))(0 := xs)\<rparr>)) (1, 0)
+               apply (rule dataplane_tracker_inv_update_outputs_outside[OF dataplane_inv _ _ G])
+                apply (simp add: fun_upd_def)
+               apply (simp add: subgraph_inv(1) raw_summary_def)
+              apply (subgoal_tac \<open>outputs_at_target (summ sg) (os(1 := (os 1)\<lparr>outpu := (outpu (os 1))(0 := xs)\<rparr>)) (1, 0)
   = outputs_at_target (summ sg) os (1, 0)\<close>)
-        apply (simp add: csets_inv(1) buffers_inv BULK_BENQ_def all_edges_def all_vertices_def neighbors_def)
-        apply (simp add: subgraph_inv(1) outputs_at_target_raw_summary)
-        apply (simp add: input_stream_inv)
-        apply (simp add: subgraph_inv os_inv(4) operator_state.defs outputs_at_target_raw_summary)
+               apply (simp add: csets_inv(1) buffers_inv BULK_BENQ_def all_edges_def all_vertices_def neighbors_def)
+               apply (simp add: subgraph_inv(1) outputs_at_target_raw_summary)
+               apply (simp add: input_stream_inv)
+              apply (simp add: subgraph_inv os_inv(4) operator_state.defs outputs_at_target_raw_summary)
         subgoal
           using label_prop_inv
           by (simp_all add: all_edges_def all_vertices_def min_label_def neighbors_def labels_inv_def labels_stable_def)
@@ -4441,8 +4806,8 @@ next
   also have G: "graph_summar_nt (summ sg) (subgraph.nxt sg) os"
     apply -
     apply (rule graph_summar_nt[simplified, OF _ subgraph_inv(1)])
-    apply (rule sym)
-    apply (rule dataflow_tree_to_graph_raw_summary)
+      apply (rule sym)
+      apply (rule dataflow_tree_to_graph_raw_summary)
     using os_inv(7) apply assumption
     using subgraph_inv(2) apply assumption
     done
@@ -4463,45 +4828,45 @@ next
         apply (erule disjE)
         subgoal
           apply (intro exI conjI)
-          apply (rule wstep_trans(1))
-          apply (rule relpowp_imp_rtranclp[
+           apply (rule wstep_trans(1))
+            apply (rule relpowp_imp_rtranclp[
                 where n="length (outpu (os 1) 0)"]) 
-          apply (rule step_set_op_steps_Out_intro[where xs="outpu (os 1) 0"  and p="(1, 0)"])
-          apply (rule steps_Tau_dataflow_op_steps_Out_intro[where xs="outpu (os 1) 0" and nid = 1 and p = 0])
-          apply (subst dataflow_tree_to_operator_def)
-          apply simp
-          apply (rule steps_map_op[where xs="map _ (outpu (os 1) 0)", rotated 2])
-          apply (rule steps_comp_op_R_Out[where xs="map _ (outpu (os 1) 0)" and p="Inr (1, 0)"])
-          apply (rule steps_Out_loop_op_intro[where xs="map _ (outpu (os 1) 0)" and p="Inr (1, 0)"])
-          apply (rule steps_map_op[where xs="map _ (outpu (os 1) 0)" , rotated 2])
-          apply (rule steps_comp_op_L_Out[where xs="map _ (outpu (os 1) 0)"])
-          apply (rule steps_map_op[where xs="map _ (outpu (os 1) 0)", rotated 2])
-          apply (rule steps_label_propagation_op_Write_Some[where ys=Nil])
-          apply simp
-          apply (rule refl)+
-          apply (simp add: os_inv(4) operator_state.defs)
-          apply (rule refl)+
-          apply force
-          apply fastforce
-          apply (rule refl)+
-          apply fastforce
-          apply (rule refl)+
-          apply fastforce
-          apply fastforce
-          apply (rule refl)+
-          apply fastforce
-          apply (rule refl)+
-          apply fastforce
-          apply (rule refl)+
-          apply (rule step_set_op_intro_Out)
-          apply (rule refl)+
-          apply force
-          apply simp
-          apply (rule refl)+
+            apply (rule step_set_op_steps_Out_intro[where xs="outpu (os 1) 0"  and p="(1, 0)"])
+              apply (rule steps_Tau_dataflow_op_steps_Out_intro[where xs="outpu (os 1) 0" and nid = 1 and p = 0])
+               apply (subst dataflow_tree_to_operator_def)
+               apply simp
+               apply (rule steps_map_op[where xs="map _ (outpu (os 1) 0)", rotated 2])
+                 apply (rule steps_comp_op_R_Out[where xs="map _ (outpu (os 1) 0)" and p="Inr (1, 0)"])
+                    apply (rule steps_Out_loop_op_intro[where xs="map _ (outpu (os 1) 0)" and p="Inr (1, 0)"])
+                       apply (rule steps_map_op[where xs="map _ (outpu (os 1) 0)" , rotated 2])
+                         apply (rule steps_comp_op_L_Out[where xs="map _ (outpu (os 1) 0)"])
+                             apply (rule steps_map_op[where xs="map _ (outpu (os 1) 0)", rotated 2])
+                              apply (rule steps_label_propagation_op_Write_Some[where ys=Nil])
+                              apply simp
+                              apply (rule refl)+
+                              apply (simp add: os_inv(4) operator_state.defs)
+                              apply (rule refl)+
+                             apply force
+                            apply fastforce
+                           apply (rule refl)+
+                         apply fastforce
+                        apply (rule refl)+
+                       apply fastforce
+                      apply fastforce
+                     apply (rule refl)+
+                 apply fastforce
+                apply (rule refl)+
+               apply fastforce
+              apply (rule refl)+
+           apply (rule step_set_op_intro_Out)
+              apply (rule refl)+
+             apply force
+            apply simp
+           apply (rule refl)+
           apply (intro relcomppI)
-          apply (rule bisim_refl)
-          defer
-          apply (rule wbisim_refl)
+            apply (rule bisim_refl)
+           defer
+           apply (rule wbisim_refl)
           apply (rule wb_upto_b_sym)
           apply (rule wb_upto_b_base)
           apply (unfold R_def[simplified])
@@ -4517,10 +4882,10 @@ next
             by (simp add: label_propagation_op_def operator_state.defs dataflow_tree_to_operator_def os_inv(1))
           subgoal premises
             apply (rule arg_cong2[where f=set_spec_op])
-            apply simp_all
+             apply simp_all
             apply (subst cUn_commute)
             apply (rule arg_cong2[where f=cUn])
-            apply simp
+             apply simp
             apply (rule cimage_cong)
             subgoal
               by (simp  del: filter.simps add: subgraph_inv outputs_at_target_raw_summary csets_inv(2) label_prop_edge_batch_def label_prop_edge_record_update_def buffers_inv operator_state.defs os_inv(4) csets_inv(1))
@@ -4592,7 +4957,7 @@ next
             using dataplane_inv[unfolded dataplane_tracker_inv_def, simplified] apply -
             apply clarsimp
             subgoal premises dt_inv for cap
-              using propagate_all_frontier_change_multiplicities_c_imp_correctnessE[OF D, of "pt_tr sg" "extract_progress 0 (subgraph.nxt sg) \<lparr>cons = consu os_input, inte = operator_state.inter os_input, prod = produ os_input\<rparr>", unfolded subgraph_inv(1), simplified]
+              using propagate_all_frontier_change_multiplicities_c_imp_correctnessE[OF D, of "pt_tr sg" "extract_progress 0 (graph_to_nxt (antichain_from_list \<circ>\<circ> raw_summary)) (snd (obtain_progress os_input))", unfolded subgraph_inv(1), simplified]
               apply -
               apply (drule meta_mp)
               subgoal
@@ -4606,7 +4971,7 @@ next
               apply (drule meta_mp)
               subgoal 
                 unfolding extract_progress_def
-                apply (clarsimp simp add: subgraph_inv(1,2) set_map_filter split_beta operator_state.defs os_inv(1) image_iff split: option.splits)
+                apply (clarsimp simp add: obtain_progress_def subgraph_inv(1,2) set_map_filter split_beta operator_state.defs os_inv(1) image_iff split: option.splits)
                 subgoal for l t
                   using loc_3_2_cases[of l]
                   using dt_inv(7)[unfolded change_deltas_inv_def]
@@ -4618,7 +4983,7 @@ next
                 subgoal for l t m
                   apply (subst frontier_less_equal_iff2[symmetric])
                   apply (rule frontier_less_equal_le_trans[rotated])
-                  apply (rule dt_inv(5)[unfolded imp_front_inv_def, rule_format, of l])
+                   apply (rule dt_inv(5)[unfolded imp_front_inv_def, rule_format, of l])
                   apply (rule dt_inv(9)[unfolded extract_prog_changes_above_impl_inv_def changes_above_impl_inv_def, simplified, rule_format, where xs=Nil and x="(l, t, m)" and nid=0, simplified])
                   apply (clarsimp simp add: obtain_progress_def subgraph_inv(1,2) set_map_filter split_beta operator_state.defs os_inv(1) image_iff split: option.splits)
                   done
@@ -4628,128 +4993,126 @@ next
                 using raw_summary_no_self_loop by auto
               apply clarsimp
               subgoal premises first_propa for c'
+
                 apply (intro exI conjI[rotated])
-                apply (intro relcomppI)
-                apply (rule bisim_refl)
-                defer
-                apply (rule wbisim_refl)
-                apply (rule wstep_trans(1))
-                apply (rule transitive_closurep_trans'(2))
+                 apply (intro relcomppI)
+                   apply (rule bisim_refl)
+                  defer
+                  apply (rule wbisim_refl)
+                 apply (rule wstep_trans(1))
+                  apply (rule transitive_closurep_trans'(2))
 
 
-                apply (rule converse_rtranclp_into_rtranclp) 
-                apply (rule step_set_op_intro_Tau_2)
-                apply simp
-                apply (rule step_Tau_dataflow_op_Out_Inl_intro[where nid=0])
-                apply (subst dataflow_tree_to_operator_def)
-                apply simp
-                apply (rule step_map_op)
-                apply (rule step_comp_op_L_Out)
-                apply (rule step_map_op)
-                apply (rule step_ooo_input_op_Write_None)
-                apply (rule refl)+
-                apply (subst obtain_progress_def)
-                apply simp
-                apply (rule refl)+
-                apply simp
-                apply fastforce
-                apply (rule refl)+
-                apply simp
-                apply (rule refl)+
+                   apply (rule converse_rtranclp_into_rtranclp) 
+                    apply (rule step_set_op_intro_Tau_2)
+                      apply simp
+                     apply (rule step_Tau_dataflow_op_Out_Inl_intro[where nid=0])
+                      apply (subst dataflow_tree_to_operator_def)
+                      apply simp
+                      apply (rule step_map_op)
+                       apply (rule step_comp_op_L_Out)
+                          apply (rule step_map_op)
+                           apply (rule step_ooo_input_op_Write_None_alt)
+                            apply (rule refl)+
+                          apply simp
+                         apply fastforce
+                        apply (rule refl)+
+                      apply simp
+                     apply (rule refl)+
 
-                apply (rule converse_rtranclp_into_rtranclp) 
-                apply (rule step_set_op_intro_Tau_2)
-                apply simp
-                apply (rule step_Tau_dataflow_op_Inp_Inl_intro)
-                apply (rule step_map_op)
-                apply (rule step_comp_op_R_Inp)
-                apply (rule step_Inp_loop_op)
-                apply (rule step_map_op)
-                apply (rule step_comp_op_L_Inp)
-                apply (rule step_map_op)
-                apply (rule step_label_propagation_op_Read_None)
-                apply (rule refl)+
-                apply simp
-                apply (rule refl)+
-                apply simp
-                apply (auto simp add: ran_def split: sum.splits option.splits prod.splits)[1]
-                apply (auto simp add: ran_def split: sum.splits option.splits prod.splits)[1]
-                apply (rule refl)+
-                apply simp
-                apply (simp add:  operator_state.defs subgraph_inv os_inv(1,2))
-                using first_propa(1)[unfolded operator_state.defs subgraph_inv os_inv(1,2), simplified] apply assumption
-                apply (rule refl)+
+                   apply (rule converse_rtranclp_into_rtranclp) 
+                    apply (rule step_set_op_intro_Tau_2)
+                      apply simp
+                     apply (rule step_Tau_dataflow_op_Inp_Inl_intro)
+                        apply (rule step_map_op)
+                         apply (rule step_comp_op_R_Inp)
+                            apply (rule step_Inp_loop_op)
+                             apply (rule step_map_op)
+                              apply (rule step_comp_op_L_Inp)
+                                apply (rule step_map_op)
+                                 apply (rule step_label_propagation_op_Read_None)
+                                  apply (rule refl)+
+                                apply simp
+                               apply (rule refl)+
+                             apply simp
+                            apply (auto simp add: ran_def split: sum.splits option.splits prod.splits)[1]
+                           apply (auto simp add: ran_def split: sum.splits option.splits prod.splits)[1]
+                          apply (rule refl)+
+                        apply simp
+                       apply (simp add:   subgraph_inv)
+                using first_propa(1) apply assumption
+                      apply (rule refl)+
 
-                apply (rule transitive_closurep_trans'(2))
-                apply (rule relpowp_imp_rtranclp[where n="n"]) 
-                apply (rule step_n_Taus_set_op)
-                apply (rule step_tau_pow_dataflow_op)
-                apply simp
-                apply (rule step_tau_pow_map_op)
-                apply (rule step_taus_L_pow_comp_op_steps_intro)
-                apply (rule step_tau_pow_map_op)
-                apply (rule step_compower_ooo_input_op_iterates_n[where p=0])
+                   apply (rule transitive_closurep_trans'(2))
+                    apply (rule relpowp_imp_rtranclp[where n="n"]) 
+                    apply (rule step_n_Taus_set_op)
+                     apply (rule step_tau_pow_dataflow_op)
+                     apply simp
+                     apply (rule step_tau_pow_map_op)
+                     apply (rule step_taus_L_pow_comp_op_steps_intro)
+                      apply (rule step_tau_pow_map_op)
+                      apply (rule step_compower_ooo_input_op_iterates_n[where p=0])
                 subgoal
                   using input_stream_inv 
-                  by (simp add: os_inv(1) operator_state.defs)
+                  by (simp add: os_inv(1) obtain_progress_def operator_state.defs)
                 subgoal
                   by simp
                 subgoal
                   using os_inv(3)
-                  by (simp add: os_inv(1) operator_state.defs)
+                  by (simp add: os_inv(1) obtain_progress_def operator_state.defs)
                 subgoal
                   using stream_move
-                  by (simp add: os_inv(1) operator_state.defs)
-                apply (rule refl)+
+                  by (simp add: os_inv(1) obtain_progress_def operator_state.defs)
+                       apply (rule refl)+
 
-                apply (rule transitive_closurep_trans'(2))
-                apply (rule relpowp_imp_rtranclp[where n="(length (outpu (os 0) 0)) + length (filter is_Data (ltaken n lxs))"]) 
-                apply (rule step_n_Taus_set_op)
-                apply (rule step_tau_pow_dataflow_op)
-                apply (rule step_tau_pow_map_op)
-                apply (rule step_tau_Out_pow_comp_op_steps_intro[where xs="map (\<lambda> (t, d). Inr (t, d)) (outpu (os 0) 0) @ map (\<lambda> ev. case ev of Data t d \<Rightarrow> Inr (Inl d, t)) (filter is_Data (ltaken n lxs))" and p="Inr (0, 0)"])
-                apply (rule steps_map_op[where xs="map (\<lambda> x. Out (Some 0) (Inr x)) (outpu (os 0) 0) @ map (\<lambda> e. case e of Data t d \<Rightarrow> Out (Some 0) (Inr (Inl d, t))) (filter is_Data (ltaken n lxs))"])
-                apply (rule refl)+
-                apply simp
+                   apply (rule transitive_closurep_trans'(2))
+                    apply (rule relpowp_imp_rtranclp[where n="(length (outpu (os 0) 0)) + length (filter is_Data (ltaken n lxs))"]) 
+                    apply (rule step_n_Taus_set_op)
+                     apply (rule step_tau_pow_dataflow_op)
+                     apply (rule step_tau_pow_map_op)
+                     apply (rule step_tau_Out_pow_comp_op_steps_intro[where xs="map (\<lambda> (t, d). Inr (t, d)) (outpu (os 0) 0) @ map (\<lambda> ev. case ev of Data t d \<Rightarrow> Inr (Inl d, t)) (filter is_Data (ltaken n lxs))" and p="Inr (0, 0)"])
+                        apply (rule steps_map_op[where xs="map (\<lambda> x. Out (Some 0) (Inr x)) (outpu (os 0) 0) @ map (\<lambda> e. case e of Data t d \<Rightarrow> Out (Some 0) (Inr (Inl d, t))) (filter is_Data (ltaken n lxs))"])
+                          apply (rule refl)+
+                         apply simp
                 subgoal
                   by (auto simp add: comp_def split: IO.splits event.splits)
-                apply (rule steps_ooo_input_op_Write_Some[where ys="Nil" and xs="outpu (os 0) 0 @ map (\<lambda> ev. case ev of Data t d \<Rightarrow> (Inl d, t)) (filter is_Data (ltaken n lxs))" and p=0])
-                apply simp
-                apply (simp add: operator_state.defs os_inv(1))
-                apply (rule refl)+
-                apply simp
+                        apply (rule steps_ooo_input_op_Write_Some[where ys="Nil" and xs="outpu (os 0) 0 @ map (\<lambda> ev. case ev of Data t d \<Rightarrow> (Inl d, t)) (filter is_Data (ltaken n lxs))" and p=0])
+                           apply simp
+                          apply (simp add: obtain_progress_def operator_state.defs os_inv(1))
+                         apply (rule refl)+
+                        apply simp
                 subgoal
                   by (auto simp add: comp_def split: IO.splits event.splits)
-                apply simp
-                apply fastforce
-                apply (rule refl)+
+                       apply simp
+                      apply fastforce
+                     apply (rule refl)+
 
-                apply (rule transitive_closurep_trans'(2))
-                apply (rule relpowp_imp_rtranclp[where n="(length (cbufs (1, 0)) + length (outpu (os 0) 0) + length (filter is_Data (ltaken n lxs)))"]) 
-                apply (rule step_n_Taus_set_op)
-                apply (rule step_tau_pow_dataflow_op)
-                apply simp
-                apply (rule step_tau_pow_map_op)
-                apply (rule step_tau_Inp_pow_comp_op_steps_intro
+                   apply (rule transitive_closurep_trans'(2))
+                    apply (rule relpowp_imp_rtranclp[where n="(length (cbufs (1, 0)) + length (outpu (os 0) 0) + length (filter is_Data (ltaken n lxs)))"]) 
+                    apply (rule step_n_Taus_set_op)
+                     apply (rule step_tau_pow_dataflow_op)
+                     apply simp
+                     apply (rule step_tau_pow_map_op)
+                     apply (rule step_tau_Inp_pow_comp_op_steps_intro
                     [where n="(length (cbufs (1, 0)) + length (outpu (os 0) 0) + length (filter is_Data (ltaken n lxs)))" and p="Inr (1, 0)" and xs="map Inr (cbufs (1, 0)) @ map Inr (outpu (os 0) 0) @ map (\<lambda> ev. case ev of Data t d \<Rightarrow> Inr (Inl d, t)) (filter is_Data (ltaken n lxs))"])
-                apply (rule steps_Inp_loop_op_intro[where p="Inr (1, 0)" and xs="map Inr (cbufs (1, 0)) @ map Inr (outpu (os 0) 0) @ map (\<lambda> ev. case ev of Data t d \<Rightarrow> Inr (Inl d, t)) (filter is_Data (ltaken n lxs))"])
-                apply (rule steps_map_op[where xs="map (\<lambda> x. Inp (Inl (Inr (1, 0))) (_ x)) (cbufs (1, 0)) @ map (\<lambda> x. Inp (Inl (Inr (1, 0))) (_ x)) (outpu (os 0) 0)  @ map (\<lambda> x. Inp (Inl (Inr (1, 0))) (_ x)) (filter is_Data (ltaken n lxs))"])
-                apply (rule refl)+
-                apply fastforce
-                apply (rule steps_comp_op_L_Inp[where xs="map Inr (cbufs (1, 0)) @ map Inr (outpu (os 0) 0) @ map (\<lambda> ev. case ev of Data t d \<Rightarrow> Inr (Inl d, t)) (filter is_Data (ltaken n lxs))"and p="Inr (1, 0)"])
-                apply (rule steps_map_op[where xs="map (\<lambda> x. Inp (Some 0) (Inr x)) (cbufs (1, 0)) @ map (\<lambda> x. Inp (Some 0) (Inr x)) (outpu (os 0) 0) @ map (\<lambda> x. Inp (Some 0) (Inr x)) (map (\<lambda> ev. case ev of Data t d \<Rightarrow> (Inl d, t)) (filter is_Data (ltaken n lxs)))" ])
-                apply (rule refl)+
+                          apply (rule steps_Inp_loop_op_intro[where p="Inr (1, 0)" and xs="map Inr (cbufs (1, 0)) @ map Inr (outpu (os 0) 0) @ map (\<lambda> ev. case ev of Data t d \<Rightarrow> Inr (Inl d, t)) (filter is_Data (ltaken n lxs))"])
+                             apply (rule steps_map_op[where xs="map (\<lambda> x. Inp (Inl (Inr (1, 0))) (_ x)) (cbufs (1, 0)) @ map (\<lambda> x. Inp (Inl (Inr (1, 0))) (_ x)) (outpu (os 0) 0)  @ map (\<lambda> x. Inp (Inl (Inr (1, 0))) (_ x)) (filter is_Data (ltaken n lxs))"])
+                               apply (rule refl)+
+                              apply fastforce
+                             apply (rule steps_comp_op_L_Inp[where xs="map Inr (cbufs (1, 0)) @ map Inr (outpu (os 0) 0) @ map (\<lambda> ev. case ev of Data t d \<Rightarrow> Inr (Inl d, t)) (filter is_Data (ltaken n lxs))"and p="Inr (1, 0)"])
+                                apply (rule steps_map_op[where xs="map (\<lambda> x. Inp (Some 0) (Inr x)) (cbufs (1, 0)) @ map (\<lambda> x. Inp (Some 0) (Inr x)) (outpu (os 0) 0) @ map (\<lambda> x. Inp (Some 0) (Inr x)) (map (\<lambda> ev. case ev of Data t d \<Rightarrow> (Inl d, t)) (filter is_Data (ltaken n lxs)))" ])
+                                  apply (rule refl)+
                 subgoal
                   by (auto simp add: comp_def split: IO.splits event.splits)
-                apply (rule steps_label_propagation_op_Read_Some[where p=0 and xs="cbufs (1, 0) @ outpu (os 0) 0 @ map (\<lambda> ev. case ev of Data t d \<Rightarrow> (Inl d, t)) (filter is_Data (ltaken n lxs))"])
-                apply (rule refl)+
-                apply simp
-                apply (rule refl)+
-                apply simp
+                                apply (rule steps_label_propagation_op_Read_Some[where p=0 and xs="cbufs (1, 0) @ outpu (os 0) 0 @ map (\<lambda> ev. case ev of Data t d \<Rightarrow> (Inl d, t)) (filter is_Data (ltaken n lxs))"])
+                                 apply (rule refl)+
+                                apply simp
+                               apply (rule refl)+
+                             apply simp
                 subgoal
                   by (auto simp add: comp_def ran_def split: sum.splits IO.splits event.splits)                
-                apply (rule refl)+
-                apply simp
+                           apply (rule refl)+
+                         apply simp
                 subgoal
                   by (auto simp add: ran_def split: sum.splits)
                 subgoal
@@ -4758,34 +5121,34 @@ next
                 subgoal
                   unfolding BULK_BENQ_def
                   by simp
-                apply (rule refl)+
+                     apply (rule refl)+
 
-                apply (rule transitive_closurep_trans'(2))
-                apply (rule relpowp_imp_rtranclp[where n="(length (input (os 1) 0)) + length (cbufs (1, 0)) + length (outpu (os 0) 0) + length (filter is_Data (ltaken n lxs))"]) 
-                apply (rule step_n_Taus_set_op)
-                apply (rule step_tau_pow_dataflow_op)
-                apply simp
-                apply (rule step_tau_pow_map_op)
-                apply (rule step_taus_R_pow_comp_op_steps_intro)
-                apply (rule step_taus_loop_op_steps_intro)
-                apply (rule step_tau_pow_map_op)
-                apply (rule step_taus_L_pow_comp_op_steps_intro)
-                apply (rule step_tau_pow_map_op)
-                apply (rule step_compower_label_propagation_op_input0_eq_alt[where msgs="input (os 1) 0 @ cbufs (1, 0) @ outpu (os 0) 0 @ map (\<lambda>ev. case ev of Data t d \<Rightarrow> (Inl d, t)) (filter is_Data (ltaken n lxs))" and ys="[]"])
+                   apply (rule transitive_closurep_trans'(2))
+                    apply (rule relpowp_imp_rtranclp[where n="(length (input (os 1) 0)) + length (cbufs (1, 0)) + length (outpu (os 0) 0) + length (filter is_Data (ltaken n lxs))"]) 
+                    apply (rule step_n_Taus_set_op)
+                     apply (rule step_tau_pow_dataflow_op)
+                     apply simp
+                     apply (rule step_tau_pow_map_op)
+                     apply (rule step_taus_R_pow_comp_op_steps_intro)
+                      apply (rule step_taus_loop_op_steps_intro)
+                       apply (rule step_tau_pow_map_op)
+                       apply (rule step_taus_L_pow_comp_op_steps_intro)
+                        apply (rule step_tau_pow_map_op)
+                        apply (rule step_compower_label_propagation_op_input0_eq_alt[where msgs="input (os 1) 0 @ cbufs (1, 0) @ outpu (os 0) 0 @ map (\<lambda>ev. case ev of Data t d \<Rightarrow> (Inl d, t)) (filter is_Data (ltaken n lxs))" and ys="[]"])
                 subgoal
                   unfolding input_fold_consumes 
                   by (simp add: os_inv(4) operator_state.defs)
-                apply simp
-                apply (simp add: os_inv(3,4) operator_state.defs)
-                apply (rule refl)+
+                          apply simp
+                         apply (simp add: os_inv(3,4) operator_state.defs)
+                        apply (rule refl)+
 
-                apply (rule transitive_closurep_trans'(2))
-                apply (rule step_Taus_set_op)
-                apply (rule step_Taus_dataflow_op_Taus_intro)
-                apply (rule step_star_map_op)
-                apply (rule step_comp_op_R_Tau_start)
-                apply (rule step_tau_pow_loop_updates_alt)
-                apply simp
+                   apply (rule transitive_closurep_trans'(2))
+                    apply (rule step_Taus_set_op)
+                     apply (rule step_Taus_dataflow_op_Taus_intro)
+                     apply (rule step_star_map_op)
+                     apply (rule step_comp_op_R_Tau_start)
+                     apply (rule step_tau_pow_loop_updates_alt)
+                           apply simp
                 subgoal
                   using os_inv(7)[unfolded raw_summary_def, rule_format, of 2,  simplified] 
                   using num2_neq(1) by force
@@ -4794,14 +5157,14 @@ next
                 subgoal
                   apply (simp only: CONSUMES_CONSUMES)
                   apply (rule label_prop_upd_inv_fst_label_prop_input0_batched_inputI)
-                  apply (simp add: operator_state.defs os_inv(4) input_CONSUMES)
+                   apply (simp add: operator_state.defs os_inv(4) input_CONSUMES)
                   apply (simp add:  label_prop_inv(5) input_CONSUMES)
                   done
                 subgoal
                   apply safe
                   subgoal for t
                     apply (rule labels_inv_fst_label_prop_input0_batched_inputI)
-                    apply (simp add: operator_state.defs os_inv(4) input_CONSUMES)
+                      apply (simp add: operator_state.defs os_inv(4) input_CONSUMES)
                     subgoal for q
                       using label_prop_inv(1) by auto
                     subgoal
@@ -4814,68 +5177,68 @@ next
                   apply (simp only: CONSUMES_CONSUMES)
                   apply (clarsimp del: disjCI simp add: input_CONSUMES split_beta image_iff simp del: fold_append)
                   sorry 
-                apply (rule refl)
+                    apply (rule refl)
 
-                apply (rule converse_rtranclp_into_rtranclp) 
-                apply (rule step_set_op_intro_Tau_2)
-                apply simp
-                apply (rule step_Tau_dataflow_op_Out_Inl_intro[where nid=0])
-                apply (rule step_map_op)
-                apply (rule step_comp_op_L_Out)
-                apply (rule step_map_op)
-                apply (rule step_ooo_input_op_Write_None_alt)
-                apply (rule refl)+
-                apply simp
-                apply force
-                apply (rule refl)+
-                apply simp
-                apply fastforce
-                apply (rule refl)+
+                   apply (rule converse_rtranclp_into_rtranclp) 
+                    apply (rule step_set_op_intro_Tau_2)
+                      apply simp
+                     apply (rule step_Tau_dataflow_op_Out_Inl_intro[where nid=0])
+                      apply (rule step_map_op)
+                       apply (rule step_comp_op_L_Out)
+                          apply (rule step_map_op)
+                           apply (rule step_ooo_input_op_Write_None_alt)
+                            apply (rule refl)+
+                          apply simp
+                         apply force
+                        apply (rule refl)+
+                      apply simp
+                     apply fastforce
+                    apply (rule refl)+
 
 
-                apply (rule converse_rtranclp_into_rtranclp) 
-                apply (rule step_set_op_intro_Tau_2)
-                apply simp
-                apply (rule step_Tau_dataflow_op_Out_Inl_intro[where nid=1])
-                apply (rule step_map_op)
-                apply (rule step_comp_op_R_Out)
-                apply (rule step_Out_loop_op)
-                apply (rule step_map_op)
-                apply (rule step_comp_op_L_Out)
-                apply (rule step_map_op)
-                apply (rule step_label_propagation_op_Write_None_alt)
-                apply (rule refl)+
-                apply simp
-                apply force
-                apply (rule refl)+
-                apply simp
-                apply force
-                apply (rule refl)+
-                apply simp
-                apply simp
-                apply (rule refl)+
+                   apply (rule converse_rtranclp_into_rtranclp) 
+                    apply (rule step_set_op_intro_Tau_2)
+                      apply simp
+                     apply (rule step_Tau_dataflow_op_Out_Inl_intro[where nid=1])
+                      apply (rule step_map_op)
+                       apply (rule step_comp_op_R_Out)
+                         apply (rule step_Out_loop_op)
+                           apply (rule step_map_op)
+                            apply (rule step_comp_op_L_Out)
+                               apply (rule step_map_op)
+                                apply (rule step_label_propagation_op_Write_None_alt)
+                                 apply (rule refl)+
+                               apply simp
+                              apply force
+                             apply (rule refl)+
+                           apply simp
+                          apply force
+                         apply (rule refl)+
+                      apply simp
+                     apply simp
+                    apply (rule refl)+
 
-                apply (rule converse_rtranclp_into_rtranclp) 
-                apply (rule step_set_op_intro_Tau_2)
-                apply simp
-                apply (rule step_Tau_dataflow_op_Out_Inl_intro[where nid=2])
-                apply (rule step_map_op)
-                apply (rule step_comp_op_R_Out)
-                apply (rule step_Out_loop_op)
-                apply (rule step_map_op)
-                apply (rule step_comp_op_R_Out)
-                apply (rule step_map_op)
-                apply (rule step_increment_op_Write_None_alt)
-                apply (rule refl)+
-                apply simp
-                apply (rule refl)+
-                apply simp
-                apply force
-                apply (rule refl)+
-                apply simp
-                apply simp
-                apply (rule refl)+
-                apply (simp only: fst_loop_updates append_assoc flip: change_multiplicities_append_alt)
+                   apply (rule converse_rtranclp_into_rtranclp) 
+                    apply (rule step_set_op_intro_Tau_2)
+                      apply simp
+                     apply (rule step_Tau_dataflow_op_Out_Inl_intro[where nid=2])
+                      apply (rule step_map_op)
+                       apply (rule step_comp_op_R_Out)
+                         apply (rule step_Out_loop_op)
+                           apply (rule step_map_op)
+                            apply (rule step_comp_op_R_Out)
+                              apply (rule step_map_op)
+                               apply (rule step_increment_op_Write_None_alt)
+                                apply (rule refl)+
+                              apply simp
+                             apply (rule refl)+
+                           apply simp
+                          apply force
+                         apply (rule refl)+
+                      apply simp
+                     apply simp
+                    apply (rule refl)+
+                   apply (simp add: flip: fold_append change_multiplicities_append_alt)
                 sorry
               done
             done
